style - indentation

ADT/MapLike.lean
@@ -43,7 +43,7 @@ open Std
 section DMapLike
 
 class DMapLike (γ : Type u) (α : Type v) (β : α → Type w) extends
-  Membership α γ, DGetElem? γ α β (fun m x => x ∈ m), Size γ where
+    Membership α γ, DGetElem? γ α β (fun m x => x ∈ m), Size γ where
   emptyWithCapacity {γ α β} : Nat → γ
   insert : γ → (x : α) → (y : β x) → γ
   erase {γ α β} : γ → α → γ
@@ -67,16 +67,16 @@ theorem DMapLike.keyEquiv.refl {γ α β} [inst : DMapLike γ α β] {m : γ} : 
   simp [keyEquiv]
 
 theorem DMapLike.keyEquiv.comm {γ₁ γ₂ α β} [inst₁ : DMapLike γ₁ α β] [inst₂ : DMapLike γ₂ α β]
-  {m₁ : γ₁} {m₂ : γ₂} : keyEquiv (β:=β) m₁ m₂ ↔ keyEquiv (β:=β) m₂ m₁ := by
+    {m₁ : γ₁} {m₂ : γ₂} : keyEquiv (β:=β) m₁ m₂ ↔ keyEquiv (β:=β) m₂ m₁ := by
   simp only [keyEquiv]
   conv => left; enter [x]; rw [Iff.comm]
 
 theorem DMapLike.keyEquiv.symm {γ₁ γ₂ α β} [inst₁ : DMapLike γ₁ α β] [inst₂ : DMapLike γ₂ α β]
-  {m₁ : γ₁} {m₂ : γ₂} : keyEquiv (β:=β) m₁ m₂ → keyEquiv (β:=β) m₂ m₁ :=
+    {m₁ : γ₁} {m₂ : γ₂} : keyEquiv (β:=β) m₁ m₂ → keyEquiv (β:=β) m₂ m₁ :=
   DMapLike.keyEquiv.comm.mp
 
 theorem DMapLike.keyEquiv.trans {γ₁ γ₂ γ₃ α β} [inst₁ : DMapLike γ₁ α β] [inst₂ : DMapLike γ₂ α β] [inst₃ : DMapLike γ₃ α β]
-  {m₁ : γ₁} {m₂ : γ₂} {m₃ : γ₃} : keyEquiv (β:=β) m₁ m₂ → keyEquiv (β:=β) m₂ m₃ → keyEquiv (β:=β) m₁ m₃ := by
+    {m₁ : γ₁} {m₂ : γ₂} {m₃ : γ₃} : keyEquiv (β:=β) m₁ m₂ → keyEquiv (β:=β) m₂ m₃ → keyEquiv (β:=β) m₁ m₃ := by
   intro h₁ h₂ x
   rw [h₁, h₂]
 
@@ -84,17 +84,17 @@ theorem DMapLike.equiv.refl {γ α β} [inst : DMapLike γ α β] {m : γ} : equ
   simp [equiv, keyEquiv]
 
 theorem DMapLike.equiv.comm {γ₁ γ₂ α β} [inst₁ : DMapLike γ₁ α β] [inst₂ : DMapLike γ₂ α β]
-  {m₁ : γ₁} {m₂ : γ₂} : equiv (β:=β) m₁ m₂ ↔ equiv (β:=β) m₂ m₁ := by
+    {m₁ : γ₁} {m₂ : γ₂} : equiv (β:=β) m₁ m₂ ↔ equiv (β:=β) m₂ m₁ := by
   simp only [equiv, keyEquiv.comm (m₁:=m₁)]
   conv => enter [1, 2, x]; rw [forall_comm]
   conv => enter [1, 2, x, h₁, h₂]; rw [Eq.comm]
 
 theorem DMapLike.equiv.symm {γ₁ γ₂ α β} [inst₁ : DMapLike γ₁ α β] [inst₂ : DMapLike γ₂ α β]
-  {m₁ : γ₁} {m₂ : γ₂} : equiv (β:=β) m₁ m₂ → equiv (β:=β) m₂ m₁ :=
+    {m₁ : γ₁} {m₂ : γ₂} : equiv (β:=β) m₁ m₂ → equiv (β:=β) m₂ m₁ :=
   DMapLike.equiv.comm.mp
 
 theorem DMapLike.equiv.trans {γ₁ γ₂ γ₃ α β} [inst₁ : DMapLike γ₁ α β] [inst₂ : DMapLike γ₂ α β] [inst₃ : DMapLike γ₃ α β]
-  {m₁ : γ₁} {m₂ : γ₂} {m₃ : γ₃} : equiv (β:=β) m₁ m₂ → equiv (β:=β) m₂ m₃ → equiv (β:=β) m₁ m₃ := by
+    {m₁ : γ₁} {m₂ : γ₂} {m₃ : γ₃} : equiv (β:=β) m₁ m₂ → equiv (β:=β) m₂ m₃ → equiv (β:=β) m₁ m₃ := by
   intro h₁ h₂; apply And.intro
   case left => intro x; rw [h₁.left, h₂.left]
   case right =>
@@ -106,26 +106,26 @@ theorem DMapLike.equiv'.refl {γ α β} [inst : DMapLike γ α β] {m : γ} : eq
   simp [equiv']
 
 theorem DMapLike.equiv'.comm {γ₁ γ₂ α β} [inst₁ : DMapLike γ₁ α β] [inst₂ : DMapLike γ₂ α β]
-  {m₁ : γ₁} {m₂ : γ₂} : equiv' (β:=β) m₁ m₂ ↔ equiv' (β:=β) m₂ m₁ := by
+    {m₁ : γ₁} {m₂ : γ₂} : equiv' (β:=β) m₁ m₂ ↔ equiv' (β:=β) m₂ m₁ := by
   simp only [equiv']
   conv => left; enter [x]; rw [Eq.comm]
 
 theorem DMapLike.equiv'.symm {γ₁ γ₂ α β} [inst₁ : DMapLike γ₁ α β] [inst₂ : DMapLike γ₂ α β]
-  {m₁ : γ₁} {m₂ : γ₂} : equiv' (β:=β) m₁ m₂ → equiv' (β:=β) m₂ m₁ :=
+    {m₁ : γ₁} {m₂ : γ₂} : equiv' (β:=β) m₁ m₂ → equiv' (β:=β) m₂ m₁ :=
   DMapLike.equiv'.comm.mp
 
 theorem DMapLike.equiv'.trans {γ₁ γ₂ γ₃ α β} [inst₁ : DMapLike γ₁ α β] [inst₂ : DMapLike γ₂ α β] [inst₃ : DMapLike γ₃ α β]
-  {m₁ : γ₁} {m₂ : γ₂} {m₃ : γ₃} : equiv' (β:=β) m₁ m₂ → equiv' (β:=β) m₂ m₃ → equiv' (β:=β) m₁ m₃ := by
+    {m₁ : γ₁} {m₂ : γ₂} {m₃ : γ₃} : equiv' (β:=β) m₁ m₂ → equiv' (β:=β) m₂ m₃ → equiv' (β:=β) m₁ m₃ := by
   intro h₁ h₂ x; rw [h₁, h₂]
 
 theorem DMapLike.keyEquiv_iff_keySubset {γ₁ γ₂ α β} [inst₁ : DMapLike γ₁ α β] [inst₂ : DMapLike γ₂ α β]
-  {m₁ : γ₁} {m₂ : γ₂} : keyEquiv (β:=β) m₁ m₂ ↔ keySubset (β:=β) m₁ m₂ ∧ keySubset (β:=β) m₂ m₁ := by
+    {m₁ : γ₁} {m₂ : γ₂} : keyEquiv (β:=β) m₁ m₂ ↔ keySubset (β:=β) m₁ m₂ ∧ keySubset (β:=β) m₂ m₁ := by
   simp only [keySubset, keyEquiv]; apply Iff.intro <;> intro h
   case mp => simp [h]
   case mpr => intro x; apply Iff.intro <;> simp_all
 
 theorem DMapLike.equiv'_iff_subset {γ₁ γ₂ α β} [inst₁ : DMapLike γ₁ α β] [inst₂ : DMapLike γ₂ α β]
-  {m₁ : γ₁} {m₂ : γ₂} : equiv' (β:=β) m₁ m₂ ↔ subset (β:=β) m₁ m₂ ∧ subset (β:=β) m₂ m₁ := by
+    {m₁ : γ₁} {m₂ : γ₂} : equiv' (β:=β) m₁ m₂ ↔ subset (β:=β) m₁ m₂ ∧ subset (β:=β) m₂ m₁ := by
   simp only [subset, equiv']; apply Iff.intro <;> intro h
   case mp => simp [h]
   case mpr =>
@@ -141,7 +141,7 @@ open DMapLike
   are uniquely determined up to `Map.equiv`
 -/
 class LawfulDMapLike (γ : Type u) (α : Type v) (β : α → Type w) [inst : DMapLike γ α β]
-  extends LawfulMemSize γ α, LawfulDGetElem γ α β (fun m x => x ∈ m) where
+    extends LawfulMemSize γ α, LawfulDGetElem γ α β (fun m x => x ∈ m) where
   not_mem_empty : ∀ {k : α} {n : Nat}, ¬ k ∈ emptyWithCapacity (self:=inst) n
   mem_iff_isSome_dGetElem? : ∀ {m : γ} {k : α}, k ∈ m ↔ m[k]ᵈ?.isSome
   dGetElem?_insert_self : ∀ {m : γ} {k : α} {v : β k}, (insert m k v)[k]ᵈ? = .some v
@@ -157,20 +157,20 @@ theorem LawfulDMapLike.not_mem_iff_dGetElem?_eq_none {γ α β} [inst : DMapLike
   rw [mem_iff_isSome_dGetElem?]; simp
 
 theorem LawfulDMapLike.mem_insert {γ α β} [inst : DMapLike γ α β] [LawfulDMapLike γ α β] {m : γ} {k a : α} {v : β k} :
-  a ∈ insert m k v ↔ (k = a) ∨ a ∈ m := by
+    a ∈ insert m k v ↔ (k = a) ∨ a ∈ m := by
   rw [mem_iff_isSome_dGetElem?]; by_cases k = a
   case pos h => cases h; simp [dGetElem?_insert_self]
   case neg h => simp only [dGetElem?_insert_ne h]; simp [← mem_iff_isSome_dGetElem?, *]
 
 theorem LawfulDMapLike.mem_erase {γ α β} [inst : DMapLike γ α β] [LawfulDMapLike γ α β] {m : γ} {k a : α} :
-  a ∈ erase (β:=β) m k ↔ k ≠ a ∧ a ∈ m := by
+    a ∈ erase (β:=β) m k ↔ k ≠ a ∧ a ∈ m := by
   rw [mem_iff_isSome_dGetElem?]; by_cases k = a
   case pos h => cases h; simp [dGetElem?_erase_self]
   case neg h => simp only [dGetElem?_erase_ne h]; simp [← mem_iff_isSome_dGetElem?, h]
 
 open Classical in
 theorem LawfulDMapLike.dGetElem?_eq_none_iff {γ α β} [inst : DMapLike γ α β] [LawfulDMapLike γ α β]
-  {c : γ} {i : α} : c[i]ᵈ? = .none ↔ i ∉ c := by
+    {c : γ} {i : α} : c[i]ᵈ? = .none ↔ i ∉ c := by
   simp only [dGetElem?_def]
   split <;> simp_all
 
@@ -180,52 +180,52 @@ theorem LawfulDMapLike.dGetElem?_eq_some_dGetElem {γ α β} [inst : DMapLike γ
   simp [dGetElem?_def, h]
 
 theorem LawfulDMapLike.dGetElem!_eq_dGetElem {γ α β} [inst : DMapLike γ α β] [LawfulDMapLike γ α β] {m : γ} {k : α} [Inhabited (β k)] (h : k ∈ m) :
-  m[k]ᵈ! = m[k]ᵈ'h := by
+    m[k]ᵈ! = m[k]ᵈ'h := by
   simp [dGetElem!_def, dGetElem?_eq_some_dGetElem h]
 
 theorem LawfulDMapLike.dGetElem!_eq_default {γ α β} [inst : DMapLike γ α β] [LawfulDMapLike γ α β] {m : γ} {k : α} [Inhabited (β k)] (h : k ∉ m) :
-  m[k]ᵈ! = default := by
+    m[k]ᵈ! = default := by
   simp [dGetElem!_def, dGetElem?_eq_none_iff.mpr h]
 
 theorem LawfulDMapLike.dGetElem!_eq_get!_dGetElem? {γ α β} [inst : DMapLike γ α β] [LawfulDMapLike γ α β] {m : γ} {k : α} [Inhabited (β k)] : m[k]ᵈ! = m[k]ᵈ?.get! := by
   simp only [dGetElem!_def]; split <;> simp [*]
 
 theorem LawfulDMapLike.dGetElem?_eq_some_dGetElem! {γ α β} [inst : DMapLike γ α β] [LawfulDMapLike γ α β] {m : γ} {k : α} [Inhabited (β k)] (h : k ∈ m) :
-  m[k]ᵈ? = .some m[k]ᵈ! := by
+    m[k]ᵈ? = .some m[k]ᵈ! := by
   simp [dGetElem?_eq_some_dGetElem h, dGetElem!_eq_dGetElem h]
 
 theorem LawfulDMapLike.dGetElem?_eq_none {γ α β} [inst : DMapLike γ α β] [LawfulDMapLike γ α β] {m : γ} {k : α} [Inhabited (β k)] (h : k ∉ m) :
-  m[k]ᵈ? = .none := by
+    m[k]ᵈ? = .none := by
   simp [dGetElem?_eq_none_iff.mpr h]
 
 theorem LawfulDMapLike.dGetElem_eq_iff_dGetElem?_eq_some {γ α β} [inst : DMapLike γ α β] [LawfulDMapLike γ α β] {m : γ} {k : α} {v : β k} (h : k ∈ m) :
-  m[k]ᵈ'h = v ↔ m[k]ᵈ? = .some v := by
+    m[k]ᵈ'h = v ↔ m[k]ᵈ? = .some v := by
   rw [dGetElem?_eq_some_dGetElem h]; simp
 
 theorem LawfulDMapLike.dGetElem_eq_of_dGetElem?_eq_some {γ α β} [inst : DMapLike γ α β] [LawfulDMapLike γ α β] {m : γ} {k : α} {v : β k}
-  (h : m[k]ᵈ? = .some v) : m[k]ᵈ'(mem_iff_dGetElem?_eq_some.mpr ⟨_, h⟩) = v := by
+    (h : m[k]ᵈ? = .some v) : m[k]ᵈ'(mem_iff_dGetElem?_eq_some.mpr ⟨_, h⟩) = v := by
   apply (LawfulDMapLike.dGetElem_eq_iff_dGetElem?_eq_some _).mpr h
 
 theorem LawfulDMapLike.dGetElem_eq_dGetElem_iff_dGetElem?_eq_dGetElem? {γ α β} [inst : DMapLike γ α β] [LawfulDMapLike γ α β] {m₁ m₂ : γ} {k : α}
-  (h₁ : k ∈ m₁) (h₂ : k ∈ m₂) : m₁[k]ᵈ'h₁ = m₂[k]ᵈ'h₂ ↔ m₁[k]ᵈ? = m₂[k]ᵈ? := by
+    (h₁ : k ∈ m₁) (h₂ : k ∈ m₂) : m₁[k]ᵈ'h₁ = m₂[k]ᵈ'h₂ ↔ m₁[k]ᵈ? = m₂[k]ᵈ? := by
   rw [dGetElem?_eq_some_dGetElem h₁, dGetElem?_eq_some_dGetElem h₂]; simp
 
 theorem LawfulDMapLike.dGetElem_insert_self {γ α β} [inst : DMapLike γ α β] [LawfulDMapLike γ α β] {m : γ} {k : α} {v : β k} :
-  (insert m k v)[k]ᵈ'(mem_insert.mpr (Or.inl rfl)) = v := by
+    (insert m k v)[k]ᵈ'(mem_insert.mpr (Or.inl rfl)) = v := by
   have hmem : k ∈ insert m k v := mem_insert.mpr (Or.inl rfl)
   have heq := dGetElem?_eq_some_dGetElem hmem
   rw [dGetElem?_insert_self] at heq
   injection heq with heq; rw [← heq]
 
 theorem LawfulDMapLike.dGetElem_insert_ne {γ α β} [inst : DMapLike γ α β] [LawfulDMapLike γ α β] {m : γ} {k a : α} {v : β k} (h₁ : a ∈ insert m k v) (h₂ : k ≠ a) :
-  (insert m k v)[a]ᵈ'h₁ = m[a]ᵈ'(Or.resolve_left (mem_insert.mp h₁) h₂) := by
+    (insert m k v)[a]ᵈ'h₁ = m[a]ᵈ'(Or.resolve_left (mem_insert.mp h₁) h₂) := by
   have heq := dGetElem?_eq_some_dGetElem h₁
   have heq' := dGetElem?_eq_some_dGetElem (Or.resolve_left (mem_insert.mp h₁) h₂)
   rw [dGetElem?_insert_ne h₂, heq'] at heq
   injection heq with heq; rw [← heq]
 
 theorem LawfulDMapLike.dGetElem_erase {γ α β} [inst : DMapLike γ α β] [LawfulDMapLike γ α β] {m : γ} {k a : α} (h' : a ∈ erase m k) :
-  (erase (β:=β) m k)[a]ᵈ'h' = m[a]ᵈ'((mem_erase.mp h').right) := by
+    (erase (β:=β) m k)[a]ᵈ'h' = m[a]ᵈ'((mem_erase.mp h').right) := by
   have heq := dGetElem?_eq_some_dGetElem h'
   have heq' := dGetElem?_eq_some_dGetElem (mem_erase.mp h').right
   by_cases k = a
@@ -235,30 +235,30 @@ theorem LawfulDMapLike.dGetElem_erase {γ α β} [inst : DMapLike γ α β] [Law
     injection heq with heq; rw [← heq]
 
 theorem LawfulDMapLike.insert_mem_keyEquiv {γ α β} [inst : DMapLike γ α β] [LawfulDMapLike γ α β]
-  {m : γ} {k : α} {v : β k} (hmem : k ∈ m) : keyEquiv (β:=β) (insert m k v) m := by
+    {m : γ} {k : α} {v : β k} (hmem : k ∈ m) : keyEquiv (β:=β) (insert m k v) m := by
   simp [keyEquiv, mem_insert, hmem]
 
 theorem LawfulDMapLike.erase_insert_not_mem_equiv {γ α β} [inst : DMapLike γ α β] [LawfulDMapLike γ α β]
-  {m : γ} {k : α} {v : β k} (hnmem : k ∉ m) : equiv (β:=β) (erase (β:=β) (insert m k v) k) m := by
+    {m : γ} {k : α} {v : β k} (hnmem : k ∉ m) : equiv (β:=β) (erase (β:=β) (insert m k v) k) m := by
   simp only [equiv, keyEquiv, mem_erase, mem_insert, dGetElem_erase]
   apply And.intro
   case left => intro x; by_cases (k = x) <;> simp_all
   case right => intro x ⟨hne, h₁⟩ h₂; simp [dGetElem_insert_ne _ hne]
 
 theorem LawfulDMapLike.erase_not_mem_equiv {γ α β} [inst : DMapLike γ α β] [LawfulDMapLike γ α β]
-  {m : γ} {k : α} (hnmem : k ∉ m) : equiv (β:=β) (erase (β:=β) m k) m := by
+    {m : γ} {k : α} (hnmem : k ∉ m) : equiv (β:=β) (erase (β:=β) m k) m := by
   simp only [equiv, keyEquiv, mem_erase, dGetElem_erase]
   apply And.intro
   case left => intro x; by_cases (k = x) <;> simp_all
   case right => simp
 
 theorem LawfulDMapLike.insert_erase_mem_keyEquiv {γ α β} [inst : DMapLike γ α β] [LawfulDMapLike γ α β]
-  {m : γ} {k : α} {v : β k} (hmem : k ∈ m) : keyEquiv (β:=β) (insert (erase (β:=β) m k) k v) m := by
+    {m : γ} {k : α} {v : β k} (hmem : k ∈ m) : keyEquiv (β:=β) (insert (erase (β:=β) m k) k v) m := by
   simp only [keyEquiv, mem_insert, mem_erase]
   intro x; by_cases (k = x) <;> simp_all
 
 theorem LawfulDMapLike.insert_erase_dGetElem_eq_equiv {γ α β} [inst : DMapLike γ α β] [LawfulDMapLike γ α β]
-  {m : γ} {k : α} {v : β k} (hmem : k ∈ m) (hget : m[k]ᵈ'hmem = v) : equiv (β:=β) (insert (erase (β:=β) m k) k v) m := by
+    {m : γ} {k : α} {v : β k} (hmem : k ∈ m) (hget : m[k]ᵈ'hmem = v) : equiv (β:=β) (insert (erase (β:=β) m k) k v) m := by
   simp only [equiv, keyEquiv, mem_insert, mem_erase]
   apply And.intro
   case left => intro x; grind
@@ -268,7 +268,7 @@ theorem LawfulDMapLike.insert_erase_dGetElem_eq_equiv {γ α β} [inst : DMapLik
     case inr hne => simp [dGetElem_insert_ne _ hne.left, dGetElem_erase]
 
 theorem LawfulDMapLike.exists_key_list {γ α β} [inst : DMapLike γ α β] [LawfulDMapLike γ α β] {m : γ} :
-  ∃ (l : List α), l.length = Size.size m ∧ l.Nodup ∧ ∀ k, k ∈ m ↔ k ∈ l := by
+    ∃ (l : List α), l.length = Size.size m ∧ l.Nodup ∧ ∀ k, k ∈ m ↔ k ∈ l := by
   generalize hsz : Size.size m = n
   induction n generalizing m
   case zero =>
@@ -295,20 +295,20 @@ noncomputable def LawfulDMapLike.exKeyList {γ α β} [inst : DMapLike γ α β]
   (exists_key_list (α:=α) (β:=β) (m:=m)).choose
 
 noncomputable def LawfulDMapLike.length_exKeyList_eq_size {γ α β} [inst : DMapLike γ α β] [LawfulDMapLike γ α β] {m : γ} :
-  (exKeyList (α:=α) (β:=β) m).length = Size.size m :=
+    (exKeyList (α:=α) (β:=β) m).length = Size.size m :=
   (Exists.choose_spec exists_key_list).left
 
 noncomputable def LawfulDMapLike.length_exKeyList_nodup {γ α β} [inst : DMapLike γ α β] [LawfulDMapLike γ α β] {m : γ} :
-  (exKeyList (α:=α) (β:=β) m).Nodup :=
+    (exKeyList (α:=α) (β:=β) m).Nodup :=
   (Exists.choose_spec exists_key_list).right.left
 
 noncomputable def LawfulDMapLike.length_exKeyList_equiv {γ α β} [inst : DMapLike γ α β] [LawfulDMapLike γ α β] {m : γ} :
-  ∀ k, k ∈ m ↔ k ∈ (exKeyList (α:=α) (β:=β) m) :=
+    ∀ k, k ∈ m ↔ k ∈ (exKeyList (α:=α) (β:=β) m) :=
   (Exists.choose_spec exists_key_list).right.right
 
 theorem LawfulDMapLike.size_le_of_keySubset {γ₁ γ₂ α β} [inst₁ : DMapLike γ₁ α β] [inst₂ : DMapLike γ₂ α β]
-  [LawfulDMapLike γ₁ α β] [LawfulDMapLike γ₂ α β] {m₁ : γ₁} {m₂ : γ₂}
-  (hsub : keySubset (β:=β) m₁ m₂) : Size.size m₁ ≤ Size.size m₂ := by
+    [LawfulDMapLike γ₁ α β] [LawfulDMapLike γ₂ α β] {m₁ : γ₁} {m₂ : γ₂}
+    (hsub : keySubset (β:=β) m₁ m₂) : Size.size m₁ ≤ Size.size m₂ := by
   let ⟨l₁, heq₁, hnd₁, hequiv₁⟩ := exists_key_list (inst:=inst₁) (m:=m₁)
   let ⟨l₂, heq₂, hnd₂, hequiv₂⟩ := exists_key_list (inst:=inst₂) (m:=m₂)
   rw [← heq₁, ← heq₂]
@@ -317,16 +317,16 @@ theorem LawfulDMapLike.size_le_of_keySubset {γ₁ γ₂ α β} [inst₁ : DMapL
   rw [← hequiv₂]; apply hsub; rw [hequiv₁]; exact hx
 
 theorem LawfulDMapLike.size_eq_of_keyEquiv {γ₁ γ₂ α β} [inst₁ : DMapLike γ₁ α β] [inst₂ : DMapLike γ₂ α β]
-  [LawfulDMapLike γ₁ α β] [LawfulDMapLike γ₂ α β] {m₁ : γ₁} {m₂ : γ₂}
-  (hequiv : keyEquiv (β:=β) m₁ m₂) : Size.size m₁ = Size.size m₂ := by
+    [LawfulDMapLike γ₁ α β] [LawfulDMapLike γ₂ α β] {m₁ : γ₁} {m₂ : γ₂}
+    (hequiv : keyEquiv (β:=β) m₁ m₂) : Size.size m₁ = Size.size m₂ := by
   rw [keyEquiv_iff_keySubset] at hequiv
   have h₁ := size_le_of_keySubset hequiv.left
   have h₂ := size_le_of_keySubset hequiv.right
   omega
 
 theorem LawfulDMapLike.keyEquiv_iff_size_eq_and_keySubset {γ₁ γ₂ α β} [inst₁ : DMapLike γ₁ α β] [inst₂ : DMapLike γ₂ α β]
-  [LawfulDMapLike γ₁ α β] [LawfulDMapLike γ₂ α β] {m₁ : γ₁} {m₂ : γ₂} :
-  keyEquiv (β:=β) m₁ m₂ ↔ Size.size m₁ = Size.size m₂ ∧ keySubset (β:=β) m₁ m₂ := by
+    [LawfulDMapLike γ₁ α β] [LawfulDMapLike γ₂ α β] {m₁ : γ₁} {m₂ : γ₂} :
+    keyEquiv (β:=β) m₁ m₂ ↔ Size.size m₁ = Size.size m₂ ∧ keySubset (β:=β) m₁ m₂ := by
   let ⟨l₁, heq₁, hnd₁, hequiv₁⟩ := exists_key_list (β:=β) (m:=m₁)
   let ⟨l₂, heq₂, hnd₂, hequiv₂⟩ := exists_key_list (β:=β) (m:=m₂)
   simp only [keyEquiv, keySubset]
@@ -337,56 +337,56 @@ theorem LawfulDMapLike.keyEquiv_iff_size_eq_and_keySubset {γ₁ γ₂ α β} [i
   apply List.perm_iff_length_eq_andsubPerm
 
 theorem LawfulDMapLike.size_insert_mem {γ α β} [inst : DMapLike γ α β] [LawfulDMapLike γ α β] {m : γ}
-  {k : α} {v : β k} (hmem : k ∈ m) : Size.size (insert m k v) = Size.size m := by
+    {k : α} {v : β k} (hmem : k ∈ m) : Size.size (insert m k v) = Size.size m := by
   apply size_eq_of_keyEquiv; apply insert_mem_keyEquiv hmem
 
 theorem LawfulDMapLike.size_insert_not_mem {γ α β} [inst : DMapLike γ α β] [LawfulDMapLike γ α β] {m : γ}
-  {k : α} {v : β k} (hnmem : k ∉ m) : Size.size (insert m k v) = Size.size m + 1 := by
+    {k : α} {v : β k} (hnmem : k ∉ m) : Size.size (insert m k v) = Size.size m + 1 := by
   have hke := erase_insert_not_mem_equiv hnmem (v:=v)
   rw [← size_eq_of_keyEquiv hke.left]; symm
   apply size_erase_mem; simp [mem_insert]
 
 theorem LawfulDMapLike.size_insert_le {γ α β} [inst : DMapLike γ α β] [LawfulDMapLike γ α β] {m : γ}
-  {k : α} {v : β k} : Size.size (insert m k v) ≤ Size.size m + 1 := by
+    {k : α} {v : β k} : Size.size (insert m k v) ≤ Size.size m + 1 := by
   by_cases k ∈ m
   case pos h => rw [size_insert_mem h]; simp
   case neg h => rw [size_insert_not_mem h]; exact .refl
 
 theorem LawfulDMapLike.le_size_insert {γ α β} [inst : DMapLike γ α β] [LawfulDMapLike γ α β] {m : γ}
-  {k : α} {v : β k} : Size.size m ≤ Size.size (insert m k v) := by
+    {k : α} {v : β k} : Size.size m ≤ Size.size (insert m k v) := by
   by_cases k ∈ m
   case pos h => rw [size_insert_mem h]; exact .refl
   case neg h => rw [size_insert_not_mem h]; simp
 
 theorem LawfulDMapLike.size_insert_gt_zero {γ α β} [inst : DMapLike γ α β] [LawfulDMapLike γ α β] {m : γ}
-  {k : α} {v : β k} : Size.size (insert m k v) > 0 := by
+    {k : α} {v : β k} : Size.size (insert m k v) > 0 := by
   by_cases k ∈ m
   case pos h => rw [size_insert_mem h]; apply LawfulMemSize.size_gt_zero_iff_exists_mem.mpr ⟨_, h⟩
   case neg h => rw [size_insert_not_mem h]; simp
 
 theorem LawfulDMapLike.size_erase_not_mem {γ α β} [inst : DMapLike γ α β] [LawfulDMapLike γ α β] {m : γ}
-  {k : α} (hnm : k ∉ m) : Size.size (erase (β:=β) m k) = Size.size m := by
+    {k : α} (hnm : k ∉ m) : Size.size (erase (β:=β) m k) = Size.size m := by
   apply size_eq_of_keyEquiv; apply (erase_not_mem_equiv hnm).left
 
 theorem LawfulDMapLike.size_erase_le {γ α β} [inst : DMapLike γ α β] [LawfulDMapLike γ α β] {m : γ}
-  {k : α} : Size.size (erase (β:=β) m k) ≤ Size.size m := by
+    {k : α} : Size.size (erase (β:=β) m k) ≤ Size.size m := by
   by_cases k ∈ m
   case pos h => have := size_erase_mem h; omega
   case neg h => rw [size_erase_not_mem h]; exact .refl
 
 theorem LawfulDMapLike.le_size_erase {γ α β} [inst : DMapLike γ α β] [LawfulDMapLike γ α β] {m : γ}
-  {k : α} : Size.size m ≤ Size.size (erase (β:=β) m k) + 1 := by
+    {k : α} : Size.size m ≤ Size.size (erase (β:=β) m k) + 1 := by
   by_cases k ∈ m
   case pos h => simp [size_erase_mem h]
   case neg h => rw [size_erase_not_mem h]; simp
 
 theorem LawfulDMapLike.dGetElem?_empty {γ α β} [inst : DMapLike γ α β] [LawfulDMapLike γ α β]
-  {capacity : Nat} {k : α} : (emptyWithCapacity (γ:=γ) (β:=β) capacity)[k]ᵈ? = .none := by
+    {capacity : Nat} {k : α} : (emptyWithCapacity (γ:=γ) (β:=β) capacity)[k]ᵈ? = .none := by
   rw [← not_mem_iff_dGetElem?_eq_none]; apply not_mem_empty
 
 theorem LawfulDMapLike.dGetElem?_insert {γ α β} [inst : DMapLike γ α β]
-  [LawfulDMapLike γ α β] [DecidableEq α] {m : γ} {k a : α} {v : β k} :
-  (insert m k v)[a]ᵈ? = if h : k = a then h ▸ some v else m[a]ᵈ? := by
+    [LawfulDMapLike γ α β] [DecidableEq α] {m : γ} {k a : α} {v : β k} :
+    (insert m k v)[a]ᵈ? = if h : k = a then h ▸ some v else m[a]ᵈ? := by
   by_cases (a ∈ insert m k v)
   case pos h =>
     rw [mem_insert] at h; by_cases (k = a)
@@ -398,23 +398,23 @@ theorem LawfulDMapLike.dGetElem?_insert {γ α β} [inst : DMapLike γ α β]
     simp [not_mem_iff_dGetElem?_eq_none.mp h.right, h.left]
 
 theorem LawfulDMapLike.dGetElem?_erase {γ α β} [inst : DMapLike γ α β]
-  [LawfulDMapLike γ α β] [DecidableEq α] {m : γ} {k a : α} :
-  (erase (β:=β) m k)[a]ᵈ? = if (k = a) then .none else m[a]ᵈ? := by
+    [LawfulDMapLike γ α β] [DecidableEq α] {m : γ} {k a : α} :
+    (erase (β:=β) m k)[a]ᵈ? = if (k = a) then .none else m[a]ᵈ? := by
   by_cases k = a
   case pos h => cases h; simp [dGetElem?_erase_self]
   case neg h => simp [dGetElem?_erase_ne h, h]
 
 open Classical in
 theorem LawfulDMapLike.dGetElem?_eq_none_iff_dGetElem?_eq_none_of_keyEquiv {γ₁ γ₂ α β}
-  [inst₁ : DMapLike γ₁ α β] [inst₂ : DMapLike γ₂ α β] [LawfulDMapLike γ₁ α β] [LawfulDMapLike γ₂ α β]
-  {m₁ : γ₁} {m₂ : γ₂} (hequiv : DMapLike.keyEquiv (β:=β) m₁ m₂)
-  (k : α) : m₁[k]ᵈ? = .none ↔ m₂[k]ᵈ? = .none := by
+    [inst₁ : DMapLike γ₁ α β] [inst₂ : DMapLike γ₂ α β] [LawfulDMapLike γ₁ α β] [LawfulDMapLike γ₂ α β]
+    {m₁ : γ₁} {m₂ : γ₂} (hequiv : DMapLike.keyEquiv (β:=β) m₁ m₂)
+    (k : α) : m₁[k]ᵈ? = .none ↔ m₂[k]ᵈ? = .none := by
   simp [dGetElem?_eq_none_iff, hequiv k]
 
 theorem LawfulDMapLike.equiv_iff_equiv' {γ₁ γ₂ α β}
-  [inst₁ : DMapLike γ₁ α β] [inst₂ : DMapLike γ₂ α β] [LawfulDMapLike γ₁ α β] [LawfulDMapLike γ₂ α β]
-  {m₁ : γ₁} {m₂ : γ₂} :
-  DMapLike.equiv (β:=β) m₁ m₂ ↔ DMapLike.equiv' (β:=β) m₁ m₂ := by
+    [inst₁ : DMapLike γ₁ α β] [inst₂ : DMapLike γ₂ α β] [LawfulDMapLike γ₁ α β] [LawfulDMapLike γ₂ α β]
+    {m₁ : γ₁} {m₂ : γ₂} :
+    DMapLike.equiv (β:=β) m₁ m₂ ↔ DMapLike.equiv' (β:=β) m₁ m₂ := by
   simp only [equiv, equiv']; apply Iff.intro
   case mp =>
     intro ⟨hk, hv⟩ x
@@ -435,13 +435,13 @@ theorem LawfulDMapLike.equiv_iff_equiv' {γ₁ γ₂ α β}
       simp only [← dGetElem?_eq_some_dGetElem, h?]
 
 theorem LawfulDMapLike.equiv_iff_subset {γ₁ γ₂ α β}
-  [inst₁ : DMapLike γ₁ α β] [inst₂ : DMapLike γ₂ α β] [LawfulDMapLike γ₁ α β] [LawfulDMapLike γ₂ α β]
-  {m₁ : γ₁} {m₂ : γ₂} : equiv (β:=β) m₁ m₂ ↔ subset (β:=β) m₁ m₂ ∧ subset (β:=β) m₂ m₁ := by
+    [inst₁ : DMapLike γ₁ α β] [inst₂ : DMapLike γ₂ α β] [LawfulDMapLike γ₁ α β] [LawfulDMapLike γ₂ α β]
+    {m₁ : γ₁} {m₂ : γ₂} : equiv (β:=β) m₁ m₂ ↔ subset (β:=β) m₁ m₂ ∧ subset (β:=β) m₂ m₁ := by
   rw [LawfulDMapLike.equiv_iff_equiv', DMapLike.equiv'_iff_subset]
 
 theorem LawfulDMapLike.keySubset_of_subset {γ₁ γ₂ α β}
-  [inst₁ : DMapLike γ₁ α β] [inst₂ : DMapLike γ₂ α β] [LawfulDMapLike γ₁ α β] [LawfulDMapLike γ₂ α β]
-  {m₁ : γ₁} {m₂ : γ₂} (h : subset (β:=β) m₁ m₂) : keySubset (β:=β) m₁ m₂ := by
+    [inst₁ : DMapLike γ₁ α β] [inst₂ : DMapLike γ₂ α β] [LawfulDMapLike γ₁ α β] [LawfulDMapLike γ₂ α β]
+    {m₁ : γ₁} {m₂ : γ₂} (h : subset (β:=β) m₁ m₂) : keySubset (β:=β) m₁ m₂ := by
   simp only [subset] at h
   intro x
   simp only [mem_iff_isSome_dGetElem?]
@@ -450,64 +450,64 @@ theorem LawfulDMapLike.keySubset_of_subset {γ₁ γ₂ α β}
   cases m₁[x]ᵈ? <;> grind
 
 theorem LawfulDMapLike.mem_congr {γ₁ γ₂ α β} [inst₁ : DMapLike γ₁ α β] [inst₂ : DMapLike γ₂ α β]
-  [LawfulDMapLike γ₁ α β] [LawfulDMapLike γ₂ α β] {m₁ : γ₁} {m₂ : γ₂}
-  (hequiv : equiv (β:=β) m₁ m₂) (x : α) : x ∈ m₁ ↔ x ∈ m₂ := hequiv.left _
+    [LawfulDMapLike γ₁ α β] [LawfulDMapLike γ₂ α β] {m₁ : γ₁} {m₂ : γ₂}
+    (hequiv : equiv (β:=β) m₁ m₂) (x : α) : x ∈ m₁ ↔ x ∈ m₂ := hequiv.left _
 
 theorem LawfulDMapLike.dGetElem?_congr {γ₁ γ₂ α β} [inst₁ : DMapLike γ₁ α β] [inst₂ : DMapLike γ₂ α β]
-  [LawfulDMapLike γ₁ α β] [LawfulDMapLike γ₂ α β] {m₁ : γ₁} {m₂ : γ₂}
-  (hequiv : equiv (β:=β) m₁ m₂) (x : α) : m₁[x]ᵈ? = m₂[x]ᵈ? :=
+    [LawfulDMapLike γ₁ α β] [LawfulDMapLike γ₂ α β] {m₁ : γ₁} {m₂ : γ₂}
+    (hequiv : equiv (β:=β) m₁ m₂) (x : α) : m₁[x]ᵈ? = m₂[x]ᵈ? :=
   LawfulDMapLike.equiv_iff_equiv'.mp hequiv _
 
 theorem LawfulDMapLike.dGetElem_congr {γ₁ γ₂ α β} [inst₁ : DMapLike γ₁ α β] [inst₂ : DMapLike γ₂ α β]
-  [LawfulDMapLike γ₁ α β] [LawfulDMapLike γ₂ α β] {m₁ : γ₁} {m₂ : γ₂}
-  (hequiv : equiv (β:=β) m₁ m₂) (x : α) (h₁ : x ∈ m₁) (h₂ : x ∈ m₂) : m₁[x]ᵈ'h₁ = m₂[x]ᵈ'h₂ := by
+    [LawfulDMapLike γ₁ α β] [LawfulDMapLike γ₂ α β] {m₁ : γ₁} {m₂ : γ₂}
+    (hequiv : equiv (β:=β) m₁ m₂) (x : α) (h₁ : x ∈ m₁) (h₂ : x ∈ m₂) : m₁[x]ᵈ'h₁ = m₂[x]ᵈ'h₂ := by
   have heq := LawfulDMapLike.dGetElem?_congr hequiv x
   simp only [dGetElem?_eq_some_dGetElem h₁,
              dGetElem?_eq_some_dGetElem h₂] at heq
   injection heq
 
 theorem LawfulDMapLike.dGetElem_congr' {γ₁ γ₂ α β} [inst₁ : DMapLike γ₁ α β] [inst₂ : DMapLike γ₂ α β]
-  [LawfulDMapLike γ₁ α β] [LawfulDMapLike γ₂ α β] {m₁ : γ₁} {m₂ : γ₂}
-  (hequiv : equiv (β:=β) m₁ m₂) (x : α) (h₁ : x ∈ m₁) : m₁[x]ᵈ'h₁ = m₂[x]ᵈ'((hequiv.left _).mp h₁) := by
+    [LawfulDMapLike γ₁ α β] [LawfulDMapLike γ₂ α β] {m₁ : γ₁} {m₂ : γ₂}
+    (hequiv : equiv (β:=β) m₁ m₂) (x : α) (h₁ : x ∈ m₁) : m₁[x]ᵈ'h₁ = m₂[x]ᵈ'((hequiv.left _).mp h₁) := by
   have heq := LawfulDMapLike.dGetElem?_congr hequiv x
   simp only [dGetElem?_eq_some_dGetElem h₁,
              dGetElem?_eq_some_dGetElem ((hequiv.left _).mp h₁)] at heq
   injection heq
 
 theorem LawfulDMapLike.dGetElem!_congr {γ₁ γ₂ α β} [inst₁ : DMapLike γ₁ α β] [inst₂ : DMapLike γ₂ α β]
-  [LawfulDMapLike γ₁ α β] [LawfulDMapLike γ₂ α β] {m₁ : γ₁} {m₂ : γ₂}
-  (hequiv : equiv (β:=β) m₁ m₂) (x : α) [Inhabited (β x)] : m₁[x]ᵈ! = m₂[x]ᵈ! := by
+    [LawfulDMapLike γ₁ α β] [LawfulDMapLike γ₂ α β] {m₁ : γ₁} {m₂ : γ₂}
+    (hequiv : equiv (β:=β) m₁ m₂) (x : α) [Inhabited (β x)] : m₁[x]ᵈ! = m₂[x]ᵈ! := by
   simp [dGetElem!_def, LawfulDMapLike.dGetElem?_congr hequiv]
 
 theorem LawfulDMapLike.emptyWithCapacity_congr {γ₁ γ₂ α β} [inst₁ : DMapLike γ₁ α β] [inst₂ : DMapLike γ₂ α β]
-  [LawfulDMapLike γ₁ α β] [LawfulDMapLike γ₂ α β] (capacity₁ capacity₂ : Nat) :
-  equiv (β:=β) (inst₂:=inst₂)
-    (emptyWithCapacity (self:=inst₁) capacity₁)
-    (emptyWithCapacity (self:=inst₂) capacity₂) := by
+    [LawfulDMapLike γ₁ α β] [LawfulDMapLike γ₂ α β] (capacity₁ capacity₂ : Nat) :
+    equiv (β:=β) (inst₂:=inst₂)
+      (emptyWithCapacity (self:=inst₁) capacity₁)
+        (emptyWithCapacity (self:=inst₂) capacity₂) := by
   rw [equiv_iff_equiv']; intro x
   simp [dGetElem?_empty]
 
 open Classical in
 theorem LawfulDMapLike.insert_congr {γ₁ γ₂ α β} [inst₁ : DMapLike γ₁ α β] [inst₂ : DMapLike γ₂ α β]
-  [LawfulDMapLike γ₁ α β] [LawfulDMapLike γ₂ α β] {m₁ : γ₁} {m₂ : γ₂}
-  (hequiv : equiv (β:=β) m₁ m₂) (k : α) (v : β k) :
-  equiv (β:=β) (insert m₁ k v) (insert m₂ k v) := by
+    [LawfulDMapLike γ₁ α β] [LawfulDMapLike γ₂ α β] {m₁ : γ₁} {m₂ : γ₂}
+    (hequiv : equiv (β:=β) m₁ m₂) (k : α) (v : β k) :
+    equiv (β:=β) (insert m₁ k v) (insert m₂ k v) := by
   rw [equiv_iff_equiv']
   intro x
   simp [dGetElem?_insert, equiv_iff_equiv'.mp hequiv _]
 
 open Classical in
 theorem LawfulDMapLike.erase_congr {γ₁ γ₂ α β} [inst₁ : DMapLike γ₁ α β] [inst₂ : DMapLike γ₂ α β]
-  [LawfulDMapLike γ₁ α β] [LawfulDMapLike γ₂ α β] {m₁ : γ₁} {m₂ : γ₂}
-  (hequiv : equiv (β:=β) m₁ m₂) (k : α) :
-  equiv (β:=β) (erase m₁ (self:=inst₁) k) (erase m₂ (self:=inst₂) k) := by
+    [LawfulDMapLike γ₁ α β] [LawfulDMapLike γ₂ α β] {m₁ : γ₁} {m₂ : γ₂}
+    (hequiv : equiv (β:=β) m₁ m₂) (k : α) :
+    equiv (β:=β) (erase m₁ (self:=inst₁) k) (erase m₂ (self:=inst₂) k) := by
   rw [equiv_iff_equiv']
   intro x
   simp [dGetElem?_erase, equiv_iff_equiv'.mp hequiv _]
 
 theorem LawfulDMapLike.size_congr {γ₁ γ₂ α β} [inst₁ : DMapLike γ₁ α β] [inst₂ : DMapLike γ₂ α β]
-  [LawfulDMapLike γ₁ α β] [LawfulDMapLike γ₂ α β] {m₁ : γ₁} {m₂ : γ₂}
-  (hequiv : equiv (β:=β) m₁ m₂) : Size.size m₁ = Size.size m₂ := by
+    [LawfulDMapLike γ₁ α β] [LawfulDMapLike γ₂ α β] {m₁ : γ₁} {m₂ : γ₂}
+    (hequiv : equiv (β:=β) m₁ m₂) : Size.size m₁ = Size.size m₂ := by
   apply LawfulDMapLike.size_eq_of_keyEquiv; exact hequiv.left
 
 instance {α β} [BEq α] [Hashable α] [LawfulBEq α] : DMapLike (DHashMap α β) α β where
@@ -650,7 +650,7 @@ section MapLike
   and computing size
 -/
 class MapLike (γ : Type u) (α : Type v) (β : Type w) extends
-  Membership α γ, GetElem? γ α β (fun m x => x ∈ m), Size γ where
+    Membership α γ, GetElem? γ α β (fun m x => x ∈ m), Size γ where
   emptyWithCapacity {γ α β} : Nat → γ
   insert : γ → α → β → γ
   erase {γ α β} : γ → α → γ
@@ -763,7 +763,7 @@ open MapLike
   are uniquely determined up to `MapLike.equiv`
 -/
 class LawfulMapLike (γ : Type u) (α : Type v) (β : Type w) [inst : MapLike γ α β]
-  extends LawfulGetElem γ α β (fun m x => x ∈ m), LawfulMemSize γ α where
+    extends LawfulGetElem γ α β (fun m x => x ∈ m), LawfulMemSize γ α where
   not_mem_empty : ∀ {k : α} {n : Nat}, ¬ k ∈ emptyWithCapacity (self:=inst) n
   mem_iff_isSome_getElem? : ∀ {m : γ} {k : α}, k ∈ m ↔ m[k]?.isSome
   getElem?_insert_self : ∀ {m : γ} {k : α} {v : β}, (insert m k v)[k]? = .some v
@@ -773,7 +773,7 @@ class LawfulMapLike (γ : Type u) (α : Type v) (β : Type w) [inst : MapLike γ
   size_erase_mem : ∀ {m : γ} {k : α}, k ∈ m → Size.size (erase (β:=β) m k) + 1 = Size.size m
 
 def LawfulMapLike_of_LawfulDMapLike {γ α β} [inst : MapLike γ α β]
-  [instL : LawfulDMapLike (inst:=DMapLike_of_MapLike inst) γ α (fun _ => β)] :
+    [instL : LawfulDMapLike (inst:=DMapLike_of_MapLike inst) γ α (fun _ => β)] :
   LawfulMapLike γ α β where
   getElem?_def := instL.dGetElem?_def
   getElem!_def c i := by
@@ -790,13 +790,13 @@ def LawfulMapLike_of_LawfulDMapLike {γ α β} [inst : MapLike γ α β]
   size_erase_mem := instL.size_erase_mem
 
 theorem LawfulMapLike_of_LawfulDMapLike' {γ α β} [inst : DMapLike γ α (fun _ => β)]
-  [instL : LawfulDMapLike γ α (fun _ => β)] :
-  LawfulMapLike (inst:=MapLike_of_DMapLike inst) γ α β :=
+    [instL : LawfulDMapLike γ α (fun _ => β)] :
+    LawfulMapLike (inst:=MapLike_of_DMapLike inst) γ α β :=
   LawfulMapLike_of_LawfulDMapLike (inst:=MapLike_of_DMapLike inst)
 
 def LawfulDMapLike_of_LawfulMapLike {γ α β} [inst : DMapLike γ α (fun _ => β)]
-  [instL : LawfulMapLike (inst:=MapLike_of_DMapLike inst) γ α β] :
-  LawfulDMapLike γ α (fun _ => β) where
+    [instL : LawfulMapLike (inst:=MapLike_of_DMapLike inst) γ α β] :
+    LawfulDMapLike γ α (fun _ => β) where
   dGetElem?_def := instL.getElem?_def
   dGetElem!_def c i := by
     intro _; have h := instL.getElem!_def c i
@@ -812,8 +812,8 @@ def LawfulDMapLike_of_LawfulMapLike {γ α β} [inst : DMapLike γ α (fun _ => 
   size_erase_mem := instL.size_erase_mem
 
 local instance LawfulDMapLike_of_LawfulMapLike' {γ α β} [inst : MapLike γ α β]
-  [instL : LawfulMapLike γ α β] :
-  LawfulDMapLike (inst:=DMapLike_of_MapLike inst) γ α (fun _ => β) :=
+    [instL : LawfulMapLike γ α β] :
+    LawfulDMapLike (inst:=DMapLike_of_MapLike inst) γ α (fun _ => β) :=
   LawfulDMapLike_of_LawfulMapLike (inst:=DMapLike_of_MapLike inst)
 
 theorem LawfulMapLike.mem_iff_getElem?_eq_some {γ α β} [inst : MapLike γ α β] [LawfulMapLike γ α β] {m : γ} {k : α} : k ∈ m ↔ ∃ v, m[k]? = .some v :=
@@ -823,16 +823,16 @@ theorem LawfulMapLike.not_mem_iff_getElem?_eq_none {γ α β} [inst : MapLike γ
   LawfulDMapLike.not_mem_iff_dGetElem?_eq_none (inst:=DMapLike_of_MapLike inst)
 
 theorem LawfulMapLike.mem_insert {γ α β} [inst : MapLike γ α β] [LawfulMapLike γ α β] {m : γ} {k a : α} {v : β} :
-  a ∈ insert m k v ↔ (k = a) ∨ a ∈ m :=
+    a ∈ insert m k v ↔ (k = a) ∨ a ∈ m :=
   LawfulDMapLike.mem_insert (inst:=DMapLike_of_MapLike inst)
 
 theorem LawfulMapLike.mem_erase {γ α β} [inst : MapLike γ α β] [LawfulMapLike γ α β] {m : γ} {k a : α} :
-  a ∈ erase (β:=β) m k ↔ k ≠ a ∧ a ∈ m :=
+    a ∈ erase (β:=β) m k ↔ k ≠ a ∧ a ∈ m :=
   LawfulDMapLike.mem_erase (inst:=DMapLike_of_MapLike inst)
 
 open Classical in
 theorem LawfulMapLike.getElem?_eq_none_iff {γ α β} [inst : MapLike γ α β] [LawfulMapLike γ α β]
-  {c : γ} {i : α} : c[i]? = .none ↔ i ∉ c := by
+    {c : γ} {i : α} : c[i]? = .none ↔ i ∉ c := by
   simp only [getElem?_def]
   split <;> simp_all
 
@@ -840,136 +840,136 @@ theorem LawfulMapLike.getElem?_eq_some_getElem {γ α β} [inst : MapLike γ α 
   LawfulDMapLike.dGetElem?_eq_some_dGetElem (inst:=DMapLike_of_MapLike inst) h
 
 theorem LawfulMapLike.getElem!_eq_getElem {γ α β} [Inhabited β] [inst : MapLike γ α β] [LawfulMapLike γ α β] {m : γ} {k : α} (h : k ∈ m) :
-  m[k]! = m[k] := LawfulDMapLike.dGetElem!_eq_dGetElem (inst:=DMapLike_of_MapLike inst) h
+    m[k]! = m[k] := LawfulDMapLike.dGetElem!_eq_dGetElem (inst:=DMapLike_of_MapLike inst) h
 
 theorem LawfulMapLike.getElem!_eq_default {γ α β} [Inhabited β] [inst : MapLike γ α β] [LawfulMapLike γ α β] {m : γ} {k : α} (h : k ∉ m) :
-  m[k]! = default := LawfulDMapLike.dGetElem!_eq_default (inst:=DMapLike_of_MapLike inst) h
+    m[k]! = default := LawfulDMapLike.dGetElem!_eq_default (inst:=DMapLike_of_MapLike inst) h
 
 theorem LawfulMapLike.getElem!_eq_get!_getElem? {γ α β} [Inhabited β] [inst : MapLike γ α β] [LawfulMapLike γ α β] {m : γ} {k : α} :
-  m[k]! = m[k]?.get! := LawfulDMapLike.dGetElem!_eq_get!_dGetElem? (inst:=DMapLike_of_MapLike inst)
+    m[k]! = m[k]?.get! := LawfulDMapLike.dGetElem!_eq_get!_dGetElem? (inst:=DMapLike_of_MapLike inst)
 
 theorem LawfulMapLike.getElem?_eq_some_getElem! {γ α β} [Inhabited β] [inst : MapLike γ α β] [LawfulMapLike γ α β] {m : γ} {k : α} (h : k ∈ m) :
-  m[k]? = .some m[k]! := LawfulDMapLike.dGetElem?_eq_some_dGetElem! (inst:=DMapLike_of_MapLike inst) h
+    m[k]? = .some m[k]! := LawfulDMapLike.dGetElem?_eq_some_dGetElem! (inst:=DMapLike_of_MapLike inst) h
 
 theorem LawfulMapLike.getElem?_eq_none {γ α β} [Inhabited β]  [inst : MapLike γ α β] [LawfulMapLike γ α β] {m : γ} {k : α} (h : k ∉ m) :
-  m[k]? = .none := LawfulDMapLike.dGetElem?_eq_none (inst:=DMapLike_of_MapLike inst) h
+    m[k]? = .none := LawfulDMapLike.dGetElem?_eq_none (inst:=DMapLike_of_MapLike inst) h
 
 theorem LawfulMapLike.getElem_eq_iff_getElem?_eq_some {γ α β} [inst : MapLike γ α β] [LawfulMapLike γ α β] {m : γ} {k : α} {v : β} (h : k ∈ m) :
-  m[k] = v ↔ m[k]? = .some v := LawfulDMapLike.dGetElem_eq_iff_dGetElem?_eq_some (inst:=DMapLike_of_MapLike inst) h
+    m[k] = v ↔ m[k]? = .some v := LawfulDMapLike.dGetElem_eq_iff_dGetElem?_eq_some (inst:=DMapLike_of_MapLike inst) h
 
 theorem LawfulMapLike.getElem_eq_of_getElem?_eq_some {γ α β} [inst : MapLike γ α β] [LawfulMapLike γ α β] {m : γ} {k : α} {v : β}
-  (h : m[k]? = .some v) : m[k]'(mem_iff_getElem?_eq_some.mpr ⟨_, h⟩) = v :=
+    (h : m[k]? = .some v) : m[k]'(mem_iff_getElem?_eq_some.mpr ⟨_, h⟩) = v :=
   LawfulDMapLike.dGetElem_eq_of_dGetElem?_eq_some (inst:=DMapLike_of_MapLike inst) h
 
 theorem LawfulMapLike.getElem_eq_getElem_iff_getElem?_eq_getElem? {γ α β} [inst : MapLike γ α β] [LawfulMapLike γ α β] {m₁ m₂ : γ} {k : α}
-  (h₁ : k ∈ m₁) (h₂ : k ∈ m₂) : m₁[k] = m₂[k] ↔ m₁[k]? = m₂[k]? :=
+    (h₁ : k ∈ m₁) (h₂ : k ∈ m₂) : m₁[k] = m₂[k] ↔ m₁[k]? = m₂[k]? :=
   LawfulDMapLike.dGetElem_eq_dGetElem_iff_dGetElem?_eq_dGetElem? (inst:=DMapLike_of_MapLike inst) h₁ h₂
 
 theorem LawfulMapLike.getElem_insert_self {γ α β} [inst : MapLike γ α β] [LawfulMapLike γ α β] {m : γ} {k : α} {v : β} :
-  (insert m k v)[k]'(mem_insert.mpr (Or.inl rfl)) = v :=
+    (insert m k v)[k]'(mem_insert.mpr (Or.inl rfl)) = v :=
   LawfulDMapLike.dGetElem_insert_self (inst:=DMapLike_of_MapLike inst)
 
 theorem LawfulMapLike.getElem_insert_ne {γ α β} [inst : MapLike γ α β] [LawfulMapLike γ α β] {m : γ} {k a : α} {v : β} (h₁ : a ∈ insert m k v) (h₂ : k ≠ a) :
-  (insert m k v)[a] = m[a]'(Or.resolve_left (mem_insert.mp h₁) h₂) :=
+    (insert m k v)[a] = m[a]'(Or.resolve_left (mem_insert.mp h₁) h₂) :=
   LawfulDMapLike.dGetElem_insert_ne (inst:=DMapLike_of_MapLike inst) h₁ h₂
 
 theorem LawfulMapLike.getElem_erase {γ α β} [inst : MapLike γ α β] [LawfulMapLike γ α β] {m : γ} {k a : α} (h' : a ∈ erase m k) :
-  (erase (β:=β) m k)[a] = m[a]'((mem_erase.mp h').right) :=
+    (erase (β:=β) m k)[a] = m[a]'((mem_erase.mp h').right) :=
   LawfulDMapLike.dGetElem_erase (inst:=DMapLike_of_MapLike inst) h'
 
 theorem LawfulMapLike.insert_mem_keyEquiv {γ α β} [inst : MapLike γ α β] [LawfulMapLike γ α β]
-  {m : γ} {k : α} {v : β} (hmem : k ∈ m) : keyEquiv (α:=α) (β:=β) (insert (self:=inst) m k v) m :=
+    {m : γ} {k : α} {v : β} (hmem : k ∈ m) : keyEquiv (α:=α) (β:=β) (insert (self:=inst) m k v) m :=
   LawfulDMapLike.insert_mem_keyEquiv (inst:=DMapLike_of_MapLike inst) hmem
 
 theorem LawfulMapLike.erase_insert_not_mem_equiv {γ α β} [inst : MapLike γ α β] [LawfulMapLike γ α β]
-  {m : γ} {k : α} {v : β} (hnmem : k ∉ m) : equiv (α:=α) (β:=β) (erase (self:=inst) (insert (self:=inst) m k v) k) m :=
+    {m : γ} {k : α} {v : β} (hnmem : k ∉ m) : equiv (α:=α) (β:=β) (erase (self:=inst) (insert (self:=inst) m k v) k) m :=
   LawfulDMapLike.erase_insert_not_mem_equiv (inst:=DMapLike_of_MapLike inst) hnmem
 
 theorem LawfulMapLike.erase_not_mem_equiv {γ α β} [inst : MapLike γ α β] [LawfulMapLike γ α β]
-  {m : γ} {k : α} (hnmem : k ∉ m) : equiv (α:=α) (β:=β) (erase (self:=inst) m k) m :=
+    {m : γ} {k : α} (hnmem : k ∉ m) : equiv (α:=α) (β:=β) (erase (self:=inst) m k) m :=
   LawfulDMapLike.erase_not_mem_equiv (inst:=DMapLike_of_MapLike inst) hnmem
 
 theorem LawfulMapLike.insert_erase_mem_keyEquiv {γ α β} [inst : MapLike γ α β] [LawfulMapLike γ α β]
-  {m : γ} {k : α} {v : β} (hmem : k ∈ m) : keyEquiv (α:=α) (β:=β) (insert (erase (self:=inst) m k) k v) m :=
+    {m : γ} {k : α} {v : β} (hmem : k ∈ m) : keyEquiv (α:=α) (β:=β) (insert (erase (self:=inst) m k) k v) m :=
   LawfulDMapLike.insert_erase_mem_keyEquiv (inst:=DMapLike_of_MapLike inst) hmem
 
 theorem LawfulMapLike.insert_erase_getElem_eq_equiv {γ α β} [inst : MapLike γ α β] [LawfulMapLike γ α β]
-  {m : γ} {k : α} {v : β} (hmem : k ∈ m) (hget : m[k] = v) : equiv (α:=α) (β:=β) (insert (erase (self:=inst) m k) k v) m :=
+    {m : γ} {k : α} {v : β} (hmem : k ∈ m) (hget : m[k] = v) : equiv (α:=α) (β:=β) (insert (erase (self:=inst) m k) k v) m :=
   LawfulDMapLike.insert_erase_dGetElem_eq_equiv (inst:=DMapLike_of_MapLike inst) hmem hget
 
 theorem LawfulMapLike.exists_key_list {γ α β} [inst : MapLike γ α β] [LawfulMapLike γ α β] {m : γ} :
-  ∃ (l : List α), l.length = Size.size m ∧ l.Nodup ∧ ∀ k, k ∈ m ↔ k ∈ l :=
+    ∃ (l : List α), l.length = Size.size m ∧ l.Nodup ∧ ∀ k, k ∈ m ↔ k ∈ l :=
   LawfulDMapLike.exists_key_list (inst:=DMapLike_of_MapLike inst)
 
 noncomputable def LawfulMapLike.exKeyList {γ α β} [inst : MapLike γ α β] [LawfulMapLike γ α β] (m : γ) : List α :=
   (exists_key_list (α:=α) (β:=β) (m:=m)).choose
 
-noncomputable def LawfulMapLike.length_exKeyList_eq_size {γ α β} [inst : MapLike γ α β] [LawfulMapLike γ α β] {m : γ} :
-  (exKeyList (α:=α) (β:=β) m).length = Size.size m :=
+theorem LawfulMapLike.length_exKeyList_eq_size {γ α β} [inst : MapLike γ α β] [LawfulMapLike γ α β] {m : γ} :
+    (exKeyList (α:=α) (β:=β) m).length = Size.size m :=
   (Exists.choose_spec exists_key_list).left
 
-noncomputable def LawfulMapLike.length_exKeyList_nodup {γ α β} [inst : MapLike γ α β] [LawfulMapLike γ α β] {m : γ} :
-  (exKeyList (α:=α) (β:=β) m).Nodup :=
+theorem LawfulMapLike.length_exKeyList_nodup {γ α β} [inst : MapLike γ α β] [LawfulMapLike γ α β] {m : γ} :
+    (exKeyList (α:=α) (β:=β) m).Nodup :=
   (Exists.choose_spec exists_key_list).right.left
 
-noncomputable def LawfulMapLike.length_exKeyList_equiv {γ α β} [inst : MapLike γ α β] [LawfulMapLike γ α β] {m : γ} :
-  ∀ k, k ∈ m ↔ k ∈ (exKeyList (α:=α) (β:=β) m) :=
+theorem LawfulMapLike.length_exKeyList_equiv {γ α β} [inst : MapLike γ α β] [LawfulMapLike γ α β] {m : γ} :
+    ∀ k, k ∈ m ↔ k ∈ (exKeyList (α:=α) (β:=β) m) :=
   (Exists.choose_spec exists_key_list).right.right
 
 theorem LawfulMapLike.size_le_of_keySubset {γ₁ γ₂ α β} [inst₁ : MapLike γ₁ α β] [inst₂ : MapLike γ₂ α β]
-  [LawfulMapLike γ₁ α β] [LawfulMapLike γ₂ α β] {m₁ : γ₁} {m₂ : γ₂}
-  (hsub : keySubset (α:=α) (β:=β) m₁ m₂) : Size.size m₁ ≤ Size.size m₂ :=
+    [LawfulMapLike γ₁ α β] [LawfulMapLike γ₂ α β] {m₁ : γ₁} {m₂ : γ₂}
+    (hsub : keySubset (α:=α) (β:=β) m₁ m₂) : Size.size m₁ ≤ Size.size m₂ :=
   LawfulDMapLike.size_le_of_keySubset (inst₁:=DMapLike_of_MapLike inst₁) (inst₂:=DMapLike_of_MapLike inst₂) hsub
 
 theorem LawfulMapLike.size_eq_of_keyEquiv {γ₁ γ₂ α β} [inst₁ : MapLike γ₁ α β] [inst₂ : MapLike γ₂ α β]
-  [LawfulMapLike γ₁ α β] [LawfulMapLike γ₂ α β] {m₁ : γ₁} {m₂ : γ₂}
-  (hequiv : keyEquiv (α:=α) (β:=β) m₁ m₂) : Size.size m₁ = Size.size m₂ :=
+    [LawfulMapLike γ₁ α β] [LawfulMapLike γ₂ α β] {m₁ : γ₁} {m₂ : γ₂}
+    (hequiv : keyEquiv (α:=α) (β:=β) m₁ m₂) : Size.size m₁ = Size.size m₂ :=
   LawfulDMapLike.size_eq_of_keyEquiv (inst₁:=DMapLike_of_MapLike inst₁) (inst₂:=DMapLike_of_MapLike inst₂) hequiv
 
 theorem LawfulMapLike.keyEquiv_iff_size_eq_and_keySubset {γ₁ γ₂ α β} [inst₁ : MapLike γ₁ α β] [inst₂ : MapLike γ₂ α β]
-  [LawfulMapLike γ₁ α β] [LawfulMapLike γ₂ α β] {m₁ : γ₁} {m₂ : γ₂} :
-  keyEquiv (α:=α) (β:=β) m₁ m₂ ↔ Size.size m₁ = Size.size m₂ ∧ keySubset (α:=α) (β:=β) m₁ m₂ :=
+    [LawfulMapLike γ₁ α β] [LawfulMapLike γ₂ α β] {m₁ : γ₁} {m₂ : γ₂} :
+    keyEquiv (α:=α) (β:=β) m₁ m₂ ↔ Size.size m₁ = Size.size m₂ ∧ keySubset (α:=α) (β:=β) m₁ m₂ :=
   LawfulDMapLike.keyEquiv_iff_size_eq_and_keySubset (inst₁:=DMapLike_of_MapLike inst₁) (inst₂:=DMapLike_of_MapLike inst₂)
 
 theorem LawfulMapLike.size_insert_mem {γ α β} [inst : MapLike γ α β] [LawfulMapLike γ α β] {m : γ}
-  {k : α} {v : β} (hmem : k ∈ m) : Size.size (insert (self:=inst) m k v) = Size.size m :=
+    {k : α} {v : β} (hmem : k ∈ m) : Size.size (insert (self:=inst) m k v) = Size.size m :=
   LawfulDMapLike.size_insert_mem (inst:=DMapLike_of_MapLike inst) hmem
 
 theorem LawfulMapLike.size_insert_not_mem {γ α β} [inst : MapLike γ α β] [LawfulMapLike γ α β] {m : γ}
-  {k : α} {v : β} (hnmem : k ∉ m) : Size.size (insert (self:=inst) m k v) = Size.size m + 1 :=
+    {k : α} {v : β} (hnmem : k ∉ m) : Size.size (insert (self:=inst) m k v) = Size.size m + 1 :=
   LawfulDMapLike.size_insert_not_mem (inst:=DMapLike_of_MapLike inst) hnmem
 
 theorem LawfulMapLike.size_insert_le {γ α β} [inst : MapLike γ α β] [LawfulMapLike γ α β] {m : γ}
-  {k : α} {v : β} : Size.size (insert m k v) ≤ Size.size m + 1 :=
+    {k : α} {v : β} : Size.size (insert m k v) ≤ Size.size m + 1 :=
   LawfulDMapLike.size_insert_le (inst:=DMapLike_of_MapLike inst)
 
 theorem LawfulMapLike.le_size_insert {γ α β} [inst : MapLike γ α β] [LawfulMapLike γ α β] {m : γ}
-  {k : α} {v : β} : Size.size m ≤ Size.size (insert m k v) :=
+    {k : α} {v : β} : Size.size m ≤ Size.size (insert m k v) :=
   LawfulDMapLike.le_size_insert (inst:=DMapLike_of_MapLike inst)
 
 theorem LawfulMapLike.size_insert_gt_zero {γ α β} [inst : MapLike γ α β] [LawfulMapLike γ α β] {m : γ}
-  {k : α} {v : β} : Size.size (insert m k v) > 0 :=
+    {k : α} {v : β} : Size.size (insert m k v) > 0 :=
   LawfulDMapLike.size_insert_gt_zero (inst:=DMapLike_of_MapLike inst)
 
 theorem LawfulMapLike.size_erase_not_mem {γ α β} [inst : MapLike γ α β] [LawfulMapLike γ α β] {m : γ}
-  {k : α} (hnm : k ∉ m) : Size.size (erase (β:=β) m k) = Size.size m :=
+    {k : α} (hnm : k ∉ m) : Size.size (erase (β:=β) m k) = Size.size m :=
   LawfulDMapLike.size_erase_not_mem (inst:=DMapLike_of_MapLike inst) hnm
 
 theorem LawfulMapLike.size_erase_le {γ α β} [inst : MapLike γ α β] [LawfulMapLike γ α β] {m : γ}
-  {k : α} : Size.size (erase (β:=β) m k) ≤ Size.size m :=
+    {k : α} : Size.size (erase (β:=β) m k) ≤ Size.size m :=
   LawfulDMapLike.size_erase_le (inst:=DMapLike_of_MapLike inst)
 
 theorem LawfulMapLike.le_size_erase {γ α β} [inst : MapLike γ α β] [LawfulMapLike γ α β] {m : γ}
-  {k : α} : Size.size m ≤ Size.size (erase (β:=β) m k) + 1 :=
+    {k : α} : Size.size m ≤ Size.size (erase (β:=β) m k) + 1 :=
   LawfulDMapLike.le_size_erase (inst:=DMapLike_of_MapLike inst)
 
 theorem LawfulMapLike.getElem?_empty {γ α β} [inst : MapLike γ α β] [LawfulMapLike γ α β]
-  {capacity : Nat} {k : α} : (emptyWithCapacity (self:=inst) capacity)[k]? = .none :=
+    {capacity : Nat} {k : α} : (emptyWithCapacity (self:=inst) capacity)[k]? = .none :=
   LawfulDMapLike.dGetElem?_empty (inst:=DMapLike_of_MapLike inst)
 
 theorem LawfulMapLike.getElem?_insert {γ α β} [inst : MapLike γ α β]
-  [LawfulMapLike γ α β] [DecidableEq α] {m : γ} {k a : α} {v : β} :
-  (insert m k v)[a]? = if (k = a) then some v else m[a]? := by
+    [LawfulMapLike γ α β] [DecidableEq α] {m : γ} {k a : α} {v : β} :
+    (insert m k v)[a]? = if (k = a) then some v else m[a]? := by
   have h := LawfulDMapLike.dGetElem?_insert (inst:=DMapLike_of_MapLike inst) (m:=m) (k:=k) (a:=a) (v:=v)
   simp only [dGetElem?, DMapLike_of_MapLike] at h
   rw [h]; split
@@ -977,31 +977,31 @@ theorem LawfulMapLike.getElem?_insert {γ α β} [inst : MapLike γ α β]
   case isFalse => rfl
 
 theorem LawfulMapLike.getElem?_erase {γ α β} [inst : MapLike γ α β]
-  [LawfulMapLike γ α β] [DecidableEq α] {m : γ} {k a : α} :
-  (erase (self:=inst) m k)[a]? = if (k = a) then .none else m[a]? :=
+    [LawfulMapLike γ α β] [DecidableEq α] {m : γ} {k a : α} :
+    (erase (self:=inst) m k)[a]? = if (k = a) then .none else m[a]? :=
   LawfulDMapLike.dGetElem?_erase (inst:=DMapLike_of_MapLike inst)
 
 open Classical in
 theorem LawfulMapLike.getElem?_eq_none_iff_getElem?_eq_none_of_keyEquiv {γ₁ γ₂ α β}
-  [inst₁ : MapLike γ₁ α β] [inst₂ : MapLike γ₂ α β] [LawfulMapLike γ₁ α β] [LawfulMapLike γ₂ α β]
-  {m₁ : γ₁} {m₂ : γ₂} (hequiv : MapLike.keyEquiv (α:=α) (β:=β) m₁ m₂)
-  (k : α) : m₁[k]? = .none ↔ m₂[k]? = .none := by
+    [inst₁ : MapLike γ₁ α β] [inst₂ : MapLike γ₂ α β] [LawfulMapLike γ₁ α β] [LawfulMapLike γ₂ α β]
+    {m₁ : γ₁} {m₂ : γ₂} (hequiv : MapLike.keyEquiv (α:=α) (β:=β) m₁ m₂)
+    (k : α) : m₁[k]? = .none ↔ m₂[k]? = .none := by
   simp [hequiv k]
 
 theorem LawfulMapLike.equiv_iff_equiv' {γ₁ γ₂ α β}
-  [inst₁ : MapLike γ₁ α β] [inst₂ : MapLike γ₂ α β] [LawfulMapLike γ₁ α β] [LawfulMapLike γ₂ α β]
-  {m₁ : γ₁} {m₂ : γ₂} :
-  MapLike.equiv (α:=α) (β:=β) m₁ m₂ ↔ MapLike.equiv' (α:=α) (β:=β) m₁ m₂ :=
+    [inst₁ : MapLike γ₁ α β] [inst₂ : MapLike γ₂ α β] [LawfulMapLike γ₁ α β] [LawfulMapLike γ₂ α β]
+    {m₁ : γ₁} {m₂ : γ₂} :
+    MapLike.equiv (α:=α) (β:=β) m₁ m₂ ↔ MapLike.equiv' (α:=α) (β:=β) m₁ m₂ :=
   LawfulDMapLike.equiv_iff_equiv' (inst₁:=DMapLike_of_MapLike inst₁) (inst₂:=DMapLike_of_MapLike inst₂)
 
 theorem LawfulMapLike.equiv_iff_subset {γ₁ γ₂ α β}
-  [inst₁ : MapLike γ₁ α β] [inst₂ : MapLike γ₂ α β] [LawfulMapLike γ₁ α β] [LawfulMapLike γ₂ α β]
-  {m₁ : γ₁} {m₂ : γ₂} : equiv (α:=α) (β:=β) m₁ m₂ ↔ subset (α:=α) (β:=β) m₁ m₂ ∧ subset (α:=α) (β:=β) m₂ m₁ := by
+    [inst₁ : MapLike γ₁ α β] [inst₂ : MapLike γ₂ α β] [LawfulMapLike γ₁ α β] [LawfulMapLike γ₂ α β]
+    {m₁ : γ₁} {m₂ : γ₂} : equiv (α:=α) (β:=β) m₁ m₂ ↔ subset (α:=α) (β:=β) m₁ m₂ ∧ subset (α:=α) (β:=β) m₂ m₁ := by
   rw [LawfulMapLike.equiv_iff_equiv', MapLike.equiv'_iff_subset]
 
 theorem LawfulMapLike.keySubset_of_subset {γ₁ γ₂ α β}
-  [inst₁ : MapLike γ₁ α β] [inst₂ : MapLike γ₂ α β] [LawfulMapLike γ₁ α β] [LawfulMapLike γ₂ α β]
-  {m₁ : γ₁} {m₂ : γ₂} (h : subset (α:=α) (β:=β) m₁ m₂) : keySubset (α:=α) (β:=β) m₁ m₂ := by
+    [inst₁ : MapLike γ₁ α β] [inst₂ : MapLike γ₂ α β] [LawfulMapLike γ₁ α β] [LawfulMapLike γ₂ α β]
+    {m₁ : γ₁} {m₂ : γ₂} (h : subset (α:=α) (β:=β) m₁ m₂) : keySubset (α:=α) (β:=β) m₁ m₂ := by
   simp only [subset] at h
   intro x
   simp only [mem_iff_isSome_getElem?]
@@ -1010,51 +1010,51 @@ theorem LawfulMapLike.keySubset_of_subset {γ₁ γ₂ α β}
   cases m₁[x]? <;> grind
 
 theorem LawfulMapLike.mem_congr {γ₁ γ₂ α β} [inst₁ : MapLike γ₁ α β] [inst₂ : MapLike γ₂ α β]
-  {m₁ : γ₁} {m₂ : γ₂} (hequiv : equiv (α:=α) (β:=β) m₁ m₂) (x : α) : x ∈ m₁ ↔ x ∈ m₂ := hequiv.left _
+    {m₁ : γ₁} {m₂ : γ₂} (hequiv : equiv (α:=α) (β:=β) m₁ m₂) (x : α) : x ∈ m₁ ↔ x ∈ m₂ := hequiv.left _
 
 theorem LawfulMapLike.getElem?_congr {γ₁ γ₂ α β} [inst₁ : MapLike γ₁ α β] [inst₂ : MapLike γ₂ α β]
-  [LawfulMapLike γ₁ α β] [LawfulMapLike γ₂ α β] {m₁ : γ₁} {m₂ : γ₂}
-  (hequiv : equiv (α:=α) (β:=β) m₁ m₂) (x : α) : m₁[x]? = m₂[x]? :=
+    [LawfulMapLike γ₁ α β] [LawfulMapLike γ₂ α β] {m₁ : γ₁} {m₂ : γ₂}
+    (hequiv : equiv (α:=α) (β:=β) m₁ m₂) (x : α) : m₁[x]? = m₂[x]? :=
   LawfulMapLike.equiv_iff_equiv'.mp hequiv _
 
 theorem LawfulMapLike.getElem_congr {γ₁ γ₂ α β} [inst₁ : MapLike γ₁ α β] [inst₂ : MapLike γ₂ α β]
-  [LawfulMapLike γ₁ α β] [LawfulMapLike γ₂ α β] {m₁ : γ₁} {m₂ : γ₂}
-  (hequiv : equiv (α:=α) (β:=β) m₁ m₂) (x : α) (h₁ : x ∈ m₁) (h₂ : x ∈ m₂) : m₁[x] = m₂[x] :=
+    [LawfulMapLike γ₁ α β] [LawfulMapLike γ₂ α β] {m₁ : γ₁} {m₂ : γ₂}
+    (hequiv : equiv (α:=α) (β:=β) m₁ m₂) (x : α) (h₁ : x ∈ m₁) (h₂ : x ∈ m₂) : m₁[x] = m₂[x] :=
   LawfulDMapLike.dGetElem_congr (inst₁:=DMapLike_of_MapLike inst₁) (inst₂:=DMapLike_of_MapLike inst₂) hequiv x h₁ h₂
 
 theorem LawfulMapLike.getElem_congr' {γ₁ γ₂ α β} [inst₁ : MapLike γ₁ α β] [inst₂ : MapLike γ₂ α β]
-  [LawfulMapLike γ₁ α β] [LawfulMapLike γ₂ α β] {m₁ : γ₁} {m₂ : γ₂}
-  (hequiv : equiv (α:=α) (β:=β) m₁ m₂) (x : α) (h₁ : x ∈ m₁) : m₁[x] = m₂[x]'((hequiv.left _).mp h₁) :=
+    [LawfulMapLike γ₁ α β] [LawfulMapLike γ₂ α β] {m₁ : γ₁} {m₂ : γ₂}
+    (hequiv : equiv (α:=α) (β:=β) m₁ m₂) (x : α) (h₁ : x ∈ m₁) : m₁[x] = m₂[x]'((hequiv.left _).mp h₁) :=
   LawfulDMapLike.dGetElem_congr' (inst₁:=DMapLike_of_MapLike inst₁) (inst₂:=DMapLike_of_MapLike inst₂) hequiv x h₁
 
 theorem LawfulMapLike.getElem!_congr {γ₁ γ₂ α β} [Inhabited β] [inst₁ : MapLike γ₁ α β] [inst₂ : MapLike γ₂ α β]
-  [LawfulMapLike γ₁ α β] [LawfulMapLike γ₂ α β] {m₁ : γ₁} {m₂ : γ₂}
-  (hequiv : equiv (α:=α) (β:=β) m₁ m₂) (x : α) : m₁[x]! = m₂[x]! :=
+    [LawfulMapLike γ₁ α β] [LawfulMapLike γ₂ α β] {m₁ : γ₁} {m₂ : γ₂}
+    (hequiv : equiv (α:=α) (β:=β) m₁ m₂) (x : α) : m₁[x]! = m₂[x]! :=
   LawfulDMapLike.dGetElem!_congr (inst₁:=DMapLike_of_MapLike inst₁) (inst₂:=DMapLike_of_MapLike inst₂) hequiv x
 
 theorem LawfulMapLike.emptyWithCapacity_congr {γ₁ γ₂ α β} [inst₁ : MapLike γ₁ α β] [inst₂ : MapLike γ₂ α β]
-  [LawfulMapLike γ₁ α β] [LawfulMapLike γ₂ α β] (capacity₁ capacity₂ : Nat) :
-  equiv (α:=α) (β:=β)
-    (emptyWithCapacity (self:=inst₁) capacity₁)
-    (emptyWithCapacity (self:=inst₂) capacity₂) :=
+    [LawfulMapLike γ₁ α β] [LawfulMapLike γ₂ α β] (capacity₁ capacity₂ : Nat) :
+    equiv (α:=α) (β:=β)
+      (emptyWithCapacity (self:=inst₁) capacity₁)
+        (emptyWithCapacity (self:=inst₂) capacity₂) :=
   LawfulDMapLike.emptyWithCapacity_congr (inst₁:=DMapLike_of_MapLike inst₁) (inst₂:=DMapLike_of_MapLike inst₂) _ _
 
 theorem LawfulMapLike.insert_congr {γ₁ γ₂ α β} [inst₁ : MapLike γ₁ α β] [inst₂ : MapLike γ₂ α β]
-  [LawfulMapLike γ₁ α β] [LawfulMapLike γ₂ α β] {m₁ : γ₁} {m₂ : γ₂}
-  (hequiv : equiv (α:=α) (β:=β) m₁ m₂) (k : α) (v : β) :
-  equiv (α:=α) (β:=β) (insert m₁ k v) (insert m₂ k v) :=
+    [LawfulMapLike γ₁ α β] [LawfulMapLike γ₂ α β] {m₁ : γ₁} {m₂ : γ₂}
+    (hequiv : equiv (α:=α) (β:=β) m₁ m₂) (k : α) (v : β) :
+    equiv (α:=α) (β:=β) (insert m₁ k v) (insert m₂ k v) :=
   LawfulDMapLike.insert_congr (inst₁:=DMapLike_of_MapLike inst₁) (inst₂:=DMapLike_of_MapLike inst₂) hequiv k v
 
 open Classical in
 theorem LawfulMapLike.erase_congr {γ₁ γ₂ α β} [inst₁ : MapLike γ₁ α β] [inst₂ : MapLike γ₂ α β]
-  [LawfulMapLike γ₁ α β] [LawfulMapLike γ₂ α β] {m₁ : γ₁} {m₂ : γ₂}
-  (hequiv : equiv (α:=α) (β:=β) m₁ m₂) (k : α) :
-  equiv (α:=α) (β:=β) (erase m₁ (self:=inst₁) k) (erase m₂ (self:=inst₂) k) :=
+    [LawfulMapLike γ₁ α β] [LawfulMapLike γ₂ α β] {m₁ : γ₁} {m₂ : γ₂}
+    (hequiv : equiv (α:=α) (β:=β) m₁ m₂) (k : α) :
+    equiv (α:=α) (β:=β) (erase m₁ (self:=inst₁) k) (erase m₂ (self:=inst₂) k) :=
   LawfulDMapLike.erase_congr (inst₁:=DMapLike_of_MapLike inst₁) (inst₂:=DMapLike_of_MapLike inst₂) hequiv k
 
 theorem LawfulMapLike.size_congr {γ₁ γ₂ α β} [inst₁ : MapLike γ₁ α β] [inst₂ : MapLike γ₂ α β]
-  [LawfulMapLike γ₁ α β] [LawfulMapLike γ₂ α β] {m₁ : γ₁} {m₂ : γ₂}
-  (hequiv : equiv (α:=α) (β:=β) m₁ m₂) : Size.size m₁ = Size.size m₂ :=
+    [LawfulMapLike γ₁ α β] [LawfulMapLike γ₂ α β] {m₁ : γ₁} {m₂ : γ₂}
+    (hequiv : equiv (α:=α) (β:=β) m₁ m₂) : Size.size m₁ = Size.size m₂ :=
   LawfulDMapLike.size_congr (inst₁:=DMapLike_of_MapLike inst₁) (inst₂:=DMapLike_of_MapLike inst₂) hequiv
 
 instance {α β} [BEq α] [Hashable α] : MapLike (HashMap α β) α β where
