ADT/Array.lean
@@ -9,8 +9,8 @@ Authors: Yicheng Qian
 -/
 
 theorem Array.push_ind {α : Type u} {motive : Array α → Prop}
-  (base : motive #[]) (ind : ∀ (head : Array α) (tail : α), motive head → motive (head.push tail)) :
-  ∀ (t : Array α), motive t := by
+    (base : motive #[]) (ind : ∀ (head : Array α) (tail : α), motive head → motive (head.push tail)) :
+    ∀ (t : Array α), motive t := by
   intro t; generalize hsz : t.size = tsz; revert t
   induction tsz
   case zero =>
@@ -24,8 +24,8 @@ theorem Array.push_ind {α : Type u} {motive : Array α → Prop}
     rw [hpush, Array.size_push] at hts; simp_all
 
 theorem Array.forall_nat_lt_size_eq
-  {α} (xs : Array α) (p : α → Prop) :
-  (∀ (i : Nat) (h : i < xs.size), p xs[i]) ↔ (∀ x ∈ xs, p x) := by
+    {α} (xs : Array α) (p : α → Prop) :
+    (∀ (i : Nat) (h : i < xs.size), p xs[i]) ↔ (∀ x ∈ xs, p x) := by
   apply Iff.intro <;> intro h
   case mp =>
     intro x hx
@@ -34,16 +34,16 @@ theorem Array.forall_nat_lt_size_eq
   case mpr => intro i _; apply h; simp
 
 theorem Array.forall_nat_lt_size_push
-  {α} (xs : Array α) (x : α) (p : α → Prop) :
-  (∀ (i : Nat) (h : i < (xs.push x).size), p (xs.push x)[i]) ↔
-    (∀ (i : Nat) (h : i < xs.size), p xs[i]) ∧ p x := by
+    {α} (xs : Array α) (x : α) (p : α → Prop) :
+    (∀ (i : Nat) (h : i < (xs.push x).size), p (xs.push x)[i]) ↔
+      (∀ (i : Nat) (h : i < xs.size), p xs[i]) ∧ p x := by
   simp only [Array.size_push, Nat.forall_lt_succ_right']
   conv => enter [1, 1, m, h]; simp [Array.getElem_push, h]
   simp
 
 theorem Array.skolemizeFinD {α} {n : Nat} (p : Fin n → α → Prop)
-  (h : ∀ (i : Fin n), ∃ (x : α), p i x) :
-  ∃ (xs : Array α) (heq : xs.size = n), ∀ (i : Fin n), p i xs[i.val] := by
+    (h : ∀ (i : Fin n), ∃ (x : α), p i x) :
+    ∃ (xs : Array α) (heq : xs.size = n), ∀ (i : Fin n), p i xs[i.val] := by
   induction n
   case zero => exists #[]; exists rfl; intro i; cases i <;> contradiction
   case succ n IH =>
@@ -58,8 +58,8 @@ theorem Array.skolemizeFinD {α} {n : Nat} (p : Fin n → α → Prop)
     case right => intro i; simp [htail i]
 
 theorem Array.skolemizeBoundedD {α} {n : Nat} (p : (i : Nat) → i < n → α → Prop)
-  (h : ∀ (i : Nat) (h : i < n), ∃ (x : α), p i h x) :
-  ∃ (xs : Array α) (heq : xs.size = n), ∀ (i : Nat) (h : i < n), p i h xs[i] := by
+    (h : ∀ (i : Nat) (h : i < n), ∃ (x : α), p i h x) :
+    ∃ (xs : Array α) (heq : xs.size = n), ∀ (i : Nat) (h : i < n), p i h xs[i] := by
   let p' : Fin n → α → Prop := fun i x => p i.val i.isLt x
   have ⟨xs, heq, h'⟩ := Array.skolemizeFinD p' (fun ⟨i, hi⟩ => h i hi)
   exists xs; exists heq; intro i hi; exact h' ⟨i, hi⟩
@@ -68,23 +68,23 @@ def Array.getShl? {α} (xs : Array α) (i : Nat) (off : Nat) : Option α :=
   if i >= off then xs[i - off]? else .none
 
 theorem Array.getShl?_eq_none_iff {α} {xs : Array α} {i : Nat} {off : Nat} :
-  xs.getShl? i off = .none ↔ i < off ∨ i ≥ off + xs.size := by
+    xs.getShl? i off = .none ↔ i < off ∨ i ≥ off + xs.size := by
   simp only [getShl?]; split
   case isTrue h => rw [Array.getElem?_eq_none_iff]; omega
   case isFalse h => simp [Nat.lt_of_not_ge h]
 
 theorem Array.getShl?_eq_some_iff {α} {xs : Array α} {i : Nat} {off : Nat} :
-  (∃ x, xs.getShl? i off = .some x) ↔ i ≥ off ∧ i < off + xs.size := by
+    (∃ x, xs.getShl? i off = .some x) ↔ i ≥ off ∧ i < off + xs.size := by
   have h := Array.getShl?_eq_none_iff (xs:=xs) (i:=i) (off:=off)
   revert h; cases (xs.getShl? i off) <;> simp <;> omega
 
 theorem Array.getShl?_isSome_iff {α} {xs : Array α} {i : Nat} {off : Nat} :
-  (xs.getShl? i off).isSome ↔ i ≥ off ∧ i < off + xs.size := by
+    (xs.getShl? i off).isSome ↔ i ≥ off ∧ i < off + xs.size := by
   rw [← Array.getShl?_eq_some_iff]
   cases xs.getShl? i off <;> simp
 
 theorem Array.getShl?_push {α} {xs : Array α} {x : α} {i : Nat} {off : Nat} :
-  (xs.push x).getShl? i off = if i = off + xs.size then .some x else xs.getShl? i off := by
+    (xs.push x).getShl? i off = if i = off + xs.size then .some x else xs.getShl? i off := by
   simp only [getShl?]; split
   case isTrue h =>
     split <;> rw [Array.getElem?_push]
@@ -100,7 +100,7 @@ theorem Array.size_singleton {α} {x : α} : #[x].size = 1 := by
   rfl
 
 theorem Array.modify_const_eq_set {α} {xs : Array α} {i : Nat} {val : α} :
-  xs.modify i (fun _ => val) = if h : i < xs.size then xs.set i val else xs := by
+    xs.modify i (fun _ => val) = if h : i < xs.size then xs.set i val else xs := by
   split
   case isTrue hlt =>
     ext
