ADT/MapAPI.lean
@@ -18,7 +18,7 @@ defined in `MapLike` with useful operations.
 section DMapAPI
 
 class DMapAPI (γ : Type u) (α : Type v) (β : α → Type w) extends
-  DMapLike γ α β, IsEmpty γ, Contains γ α where
+    DMapLike γ α β, IsEmpty γ, Contains γ α where
   insertIfNew : γ → (a : α) → β a → γ
   containsThenInsert : γ → (a : α) → β a → Bool × γ
   containsThenInsertIfNew : γ → (a : α) → β a → Bool × γ
@@ -29,8 +29,8 @@ class DMapAPI (γ : Type u) (α : Type v) (β : α → Type w) extends
 
 open DMapAPI DMapLike
 
-class LawfulDMapAPI (γ : Type u) (α : Type v) (β : α → Type w) [inst : DMapAPI γ α β]
-  extends LawfulDMapLike γ α β, LawfulIsEmptySize γ, LawfulContainsMem γ α where
+class LawfulDMapAPI (γ : Type u) (α : Type v) (β : α → Type w) [inst : DMapAPI γ α β] extends
+    LawfulDMapLike γ α β, LawfulIsEmptySize γ, LawfulContainsMem γ α where
   dGetElem?_insertIfNew_self {m : γ} {k : α} {v : β k} (h : k ∉ m) :
     (insertIfNew m k v)[k]ᵈ? = .some v
   dGetElem?_insertIfNew_ne {m : γ} {k a : α} {v : β k} (h : k ≠ a ∨ k ∈ m) :
@@ -56,52 +56,52 @@ namespace LawfulDMapAPI
   open LawfulDMapLike
 
   theorem isEmpty_congr {γ₁ γ₂ α β} [inst₁ : DMapAPI γ₁ α β] [inst₂ : DMapAPI γ₂ α β]
-    [LawfulDMapAPI γ₁ α β] [LawfulDMapAPI γ₂ α β] {m₁ : γ₁} {m₂ : γ₂}
-    (hequiv : equiv (β:=β) m₁ m₂) : IsEmpty.isEmpty m₁ = IsEmpty.isEmpty m₂ := by
+      [LawfulDMapAPI γ₁ α β] [LawfulDMapAPI γ₂ α β] {m₁ : γ₁} {m₂ : γ₂}
+      (hequiv : equiv (β:=β) m₁ m₂) : IsEmpty.isEmpty m₁ = IsEmpty.isEmpty m₂ := by
     rw [Bool.eq_iff_iff]
     simp only [LawfulIsEmptySize.isEmpty_iff_size_eq_zero]
     rw [size_congr hequiv]
 
   theorem isEmpty_erase {γ α β} [inst : DMapAPI γ α β] [LawfulDMapAPI γ α β]
-    {m : γ} {k : α} : IsEmpty.isEmpty (erase (β:=β) m k) = (IsEmpty.isEmpty m || (Size.size m == 1 && Contains.contains m k)) := by
+      {m : γ} {k : α} : IsEmpty.isEmpty (erase (β:=β) m k) = (IsEmpty.isEmpty m || (Size.size m == 1 && Contains.contains m k)) := by
     rw [Bool.eq_iff_iff]
     simp only [Bool.or_eq_true, Bool.and_eq_true, beq_iff_eq,
                LawfulContainsMem.contains_iff_mem, LawfulIsEmptySize.isEmpty_iff_size_eq_zero]
     grind [size_erase_mem, size_erase_not_mem]
 
   theorem isEmpty_insert_eq_false {γ α β} [inst : DMapAPI γ α β] [LawfulDMapAPI γ α β]
-    {m : γ} {k : α} {v : β k} : IsEmpty.isEmpty (insert m k v) = false := by
+      {m : γ} {k : α} {v : β k} : IsEmpty.isEmpty (insert m k v) = false := by
     rw [LawfulIsEmptySize.isEmpty_eq_false_iff_size_gt_zero]
     apply size_insert_gt_zero
 
   theorem contains_congr {γ₁ γ₂ α β} [inst₁ : DMapAPI γ₁ α β] [inst₂ : DMapAPI γ₂ α β]
-    [LawfulDMapAPI γ₁ α β] [LawfulDMapAPI γ₂ α β] {m₁ : γ₁} {m₂ : γ₂}
-    (hequiv : equiv (β:=β) m₁ m₂) (k : α) : Contains.contains m₁ k = Contains.contains m₂ k := by
+      [LawfulDMapAPI γ₁ α β] [LawfulDMapAPI γ₂ α β] {m₁ : γ₁} {m₂ : γ₂}
+      (hequiv : equiv (β:=β) m₁ m₂) (k : α) : Contains.contains m₁ k = Contains.contains m₂ k := by
     rw [Bool.eq_iff_iff]
     simp only [LawfulContainsMem.contains_iff_mem]
     rw [mem_congr hequiv]
 
   theorem not_contains_iff_not_mem {γ α β} [inst : DMapAPI γ α β] [LawfulDMapAPI γ α β]
-    {m : γ} {k : α} : Contains.contains m k = false ↔ k ∉ m := by
+      {m : γ} {k : α} : Contains.contains m k = false ↔ k ∉ m := by
     grind [LawfulContainsMem.contains_iff_mem]
 
   theorem isEmpty_iff_forall_not_mem {γ α β} [inst : DMapAPI γ α β] [LawfulDMapAPI γ α β]
-    {m : γ} : IsEmpty.isEmpty m ↔ ∀ (x : α), x ∉ m := by
+      {m : γ} : IsEmpty.isEmpty m ↔ ∀ (x : α), x ∉ m := by
     rw [LawfulIsEmptySize.isEmpty_iff_size_eq_zero, LawfulMemSize.size_zero_iff_forall_not_mem (α:=α)]
 
   theorem insertIfNew_equiv_of_mem {γ α β} [inst : DMapAPI γ α β] [LawfulDMapAPI γ α β]
-    {m : γ} {k : α} {v : β k} (h : k ∈ m) : equiv (β:=β) (insertIfNew m k v) m := by
+      {m : γ} {k : α} {v : β k} (h : k ∈ m) : equiv (β:=β) (insertIfNew m k v) m := by
     simp only [equiv_iff_equiv', equiv']
     grind [dGetElem?_insertIfNew_ne]
 
   open Classical in
   theorem insertIfNew_equiv_of_not_mem {γ α β} [inst : DMapAPI γ α β] [LawfulDMapAPI γ α β]
-    {m : γ} {k : α} {v : β k} (h : k ∉ m) : equiv (β:=β) (insertIfNew m k v) (insert m k v) := by
+      {m : γ} {k : α} {v : β k} (h : k ∉ m) : equiv (β:=β) (insertIfNew m k v) (insert m k v) := by
     simp only [equiv_iff_equiv', equiv', dGetElem?_insert]
     grind [dGetElem?_insertIfNew_ne, dGetElem?_insertIfNew_self]
 
   theorem insertIfNew_equiv {γ α β} [inst : DMapAPI γ α β] [LawfulDMapAPI γ α β]
-    {m : γ} {k : α} {v : β k} : equiv (β:=β) (insertIfNew m k v) (if Contains.contains m k then m else insert m k v) := by
+      {m : γ} {k : α} {v : β k} : equiv (β:=β) (insertIfNew m k v) (if Contains.contains m k then m else insert m k v) := by
     split
     case isTrue h =>
       apply insertIfNew_equiv_of_mem; apply LawfulContainsMem.contains_iff_mem.mp h
@@ -109,9 +109,9 @@ namespace LawfulDMapAPI
       apply insertIfNew_equiv_of_not_mem; grind [LawfulContainsMem.contains_iff_mem]
 
   theorem insertIfNew_congr {γ₁ γ₂ α β} [inst₁ : DMapAPI γ₁ α β] [inst₂ : DMapAPI γ₂ α β]
-    [LawfulDMapAPI γ₁ α β] [LawfulDMapAPI γ₂ α β] {m₁ : γ₁} {m₂ : γ₂}
-    (hequiv : equiv (β:=β) m₁ m₂) (k : α) (v : β k) :
-    equiv (β:=β) (insertIfNew m₁ k v) (insertIfNew m₂ k v) := by
+      [LawfulDMapAPI γ₁ α β] [LawfulDMapAPI γ₂ α β] {m₁ : γ₁} {m₂ : γ₂}
+      (hequiv : equiv (β:=β) m₁ m₂) (k : α) (v : β k) :
+      equiv (β:=β) (insertIfNew m₁ k v) (insertIfNew m₂ k v) := by
     apply equiv.trans insertIfNew_equiv
     apply equiv.trans _ (equiv.symm insertIfNew_equiv)
     rw [contains_congr hequiv]; cases (Contains.contains m₂ k)
@@ -119,69 +119,69 @@ namespace LawfulDMapAPI
     case true => simp [*]
 
   theorem size_insertIfNew_mem {γ α β} [inst : DMapAPI γ α β] [LawfulDMapAPI γ α β]
-    {m : γ} {k : α} {v : β k} (h : k ∈ m) : Size.size (insertIfNew m k v) = Size.size m := by
+      {m : γ} {k : α} {v : β k} (h : k ∈ m) : Size.size (insertIfNew m k v) = Size.size m := by
     rw [size_congr (insertIfNew_equiv_of_mem h)]
 
   theorem size_insertIfNew_not_mem {γ α β} [inst : DMapAPI γ α β] [LawfulDMapAPI γ α β]
-    {m : γ} {k : α} {v : β k} (h : k ∉ m) : Size.size (insertIfNew m k v) = Size.size m + 1 := by
+      {m : γ} {k : α} {v : β k} (h : k ∉ m) : Size.size (insertIfNew m k v) = Size.size m + 1 := by
     rw [size_congr (insertIfNew_equiv_of_not_mem h), size_insert_not_mem h]
 
   theorem size_insertIfNew {γ α β} [inst : DMapAPI γ α β] [LawfulDMapAPI γ α β]
-    {m : γ} {k : α} [Decidable (k ∈ m)] {v : β k} : Size.size (insertIfNew m k v) = if k ∈ m then Size.size m else Size.size m + 1 := by
+      {m : γ} {k : α} [Decidable (k ∈ m)] {v : β k} : Size.size (insertIfNew m k v) = if k ∈ m then Size.size m else Size.size m + 1 := by
     grind [size_insertIfNew_mem, size_insertIfNew_not_mem]
 
   theorem mem_insertIfNew' {γ α β} [inst : DMapAPI γ α β] [LawfulDMapAPI γ α β]
-    {m : γ} {k a : α} {v : β k} : a ∈ DMapAPI.insertIfNew m k v ↔ k = a ∨ a ∈ m := by
+      {m : γ} {k a : α} {v : β k} : a ∈ DMapAPI.insertIfNew m k v ↔ k = a ∨ a ∈ m := by
     rw [mem_congr insertIfNew_equiv]
     grind [mem_insert, LawfulContainsMem.contains_iff_mem]
 
   theorem mem_insertIfNew {γ α β} [BEq α] [LawfulBEq α] [inst : DMapAPI γ α β] [LawfulDMapAPI γ α β]
-    {m : γ} {k a : α} {v : β k} : a ∈ DMapAPI.insertIfNew m k v ↔ k == a ∨ a ∈ m := by
+      {m : γ} {k a : α} {v : β k} : a ∈ DMapAPI.insertIfNew m k v ↔ k == a ∨ a ∈ m := by
     simp [mem_insertIfNew']
 
   theorem mem_of_mem_insertIfNew' {γ α β} [inst : DMapAPI γ α β] [LawfulDMapAPI γ α β] {m : γ} {k a : α} {v : β k} :
-    a ∈ insertIfNew m k v → k ≠ a ∨ k ∈ m → a ∈ m := by
+      a ∈ insertIfNew m k v → k ≠ a ∨ k ∈ m → a ∈ m := by
     rw [mem_insertIfNew']; grind
 
   theorem contains_insertIfNew {γ α β} [inst : DMapAPI γ α β] [LawfulDMapAPI γ α β]
-    {m : γ} {k a : α} {v : β k} : Contains.contains (DMapAPI.insertIfNew m k v) a ↔ k = a ∨ a ∈ m := by
+      {m : γ} {k a : α} {v : β k} : Contains.contains (DMapAPI.insertIfNew m k v) a ↔ k = a ∨ a ∈ m := by
     simp [LawfulContainsMem.contains_iff_mem, mem_insertIfNew']
 
   theorem dGetElem_insertIfNew_ne {γ α β} [inst : DMapAPI γ α β] [LawfulDMapAPI γ α β]
-    {m : γ} {k a : α} {v : β k} {h₁ : a ∈ insertIfNew m k v} {h₂ : k ≠ a ∨ k ∈ m} :
-    (insertIfNew m k v)[a]ᵈ'h₁ = m[a]ᵈ'(mem_of_mem_insertIfNew' h₁ h₂) := by
+      {m : γ} {k a : α} {v : β k} {h₁ : a ∈ insertIfNew m k v} {h₂ : k ≠ a ∨ k ∈ m} :
+      (insertIfNew m k v)[a]ᵈ'h₁ = m[a]ᵈ'(mem_of_mem_insertIfNew' h₁ h₂) := by
     rw [dGetElem_eq_dGetElem_iff_dGetElem?_eq_dGetElem?, dGetElem?_insertIfNew_ne h₂]
 
   theorem dGetElem_insertIfNew_ne' {γ α β} [inst : DMapAPI γ α β] [LawfulDMapAPI γ α β]
-    {m : γ} {k a : α} {v : β k} {h : a ∈ m} :
-    (insertIfNew m k v)[a]ᵈ'(mem_insertIfNew'.mpr (Or.inr h)) = m[a]ᵈ'h := by
+      {m : γ} {k a : α} {v : β k} {h : a ∈ m} :
+      (insertIfNew m k v)[a]ᵈ'(mem_insertIfNew'.mpr (Or.inr h)) = m[a]ᵈ'h := by
     rw [dGetElem_eq_dGetElem_iff_dGetElem?_eq_dGetElem?, dGetElem?_insertIfNew_ne]; grind
 
   theorem dGetElem_insertIfNew_self {γ α β} [inst : DMapAPI γ α β] [LawfulDMapAPI γ α β]
-    {m : γ} {k: α} {v : β k} {h : k ∉ m} :
-    (insertIfNew m k v)[k]ᵈ'(by simp [mem_insertIfNew']) = v := by
+      {m : γ} {k: α} {v : β k} {h : k ∉ m} :
+      (insertIfNew m k v)[k]ᵈ'(by simp [mem_insertIfNew']) = v := by
     rw [dGetElem_eq_iff_dGetElem?_eq_some, dGetElem?_insertIfNew_self h]
 
   theorem dGetElem!_insertIfNew_ne {γ α β} [inst : DMapAPI γ α β] [LawfulDMapAPI γ α β]
-    {m : γ} {k a : α} [Inhabited (β a)] {v : β k} {h : k ≠ a ∨ k ∈ m} :
-    (insertIfNew m k v)[a]ᵈ! = m[a]ᵈ! := by
+      {m : γ} {k a : α} [Inhabited (β a)] {v : β k} {h : k ≠ a ∨ k ∈ m} :
+      (insertIfNew m k v)[a]ᵈ! = m[a]ᵈ! := by
     simp [dGetElem!_eq_get!_dGetElem?, dGetElem?_insertIfNew_ne h]
 
   theorem dGetElem!_insertIfNew_self {γ α β} [inst : DMapAPI γ α β] [LawfulDMapAPI γ α β]
-    {m : γ} {k : α} [Inhabited (β k)] {v : β k} {h : k ∉ m} :
-    (insertIfNew m k v)[k]ᵈ! = v := by
+      {m : γ} {k : α} [Inhabited (β k)] {v : β k} {h : k ∉ m} :
+      (insertIfNew m k v)[k]ᵈ! = v := by
     simp [dGetElem!_eq_get!_dGetElem?, dGetElem?_insertIfNew_self h]
 
   theorem filter_congr {γ₁ γ₂ α β} [inst₁ : DMapAPI γ₁ α β] [inst₂ : DMapAPI γ₂ α β]
-    [LawfulDMapAPI γ₁ α β] [LawfulDMapAPI γ₂ α β] {m₁ : γ₁} {m₂ : γ₂}
-    (hequiv : equiv (β:=β) m₁ m₂) (f : (a : α) → β a → Bool) :
-    equiv (β:=β) (filter f m₁) (filter f m₂) := by
+      [LawfulDMapAPI γ₁ α β] [LawfulDMapAPI γ₂ α β] {m₁ : γ₁} {m₂ : γ₂}
+      (hequiv : equiv (β:=β) m₁ m₂) (f : (a : α) → β a → Bool) :
+      equiv (β:=β) (filter f m₁) (filter f m₂) := by
     rw [equiv_iff_equiv']; intro x
     simp only [dGetElem?_filter, dGetElem?_congr hequiv]
 
   theorem mem_filter {γ α β} [inst : DMapAPI γ α β] [LawfulDMapAPI γ α β]
-    {m : γ} {f : (a : α) → β a → Bool} {k : α} :
-    k ∈ filter f m ↔ ∃ h, f k (m[k]ᵈ'h) = true := by
+      {m : γ} {f : (a : α) → β a → Bool} {k : α} :
+      k ∈ filter f m ↔ ∃ h, f k (m[k]ᵈ'h) = true := by
     rw [mem_iff_dGetElem?_eq_some, dGetElem?_filter]
     simp only [Option.filter]; split
     case h_1 heq =>
@@ -190,60 +190,60 @@ namespace LawfulDMapAPI
       simp [not_mem_iff_dGetElem?_eq_none.mpr heq]
 
   theorem mem_of_mem_filter {γ α β} [inst : DMapAPI γ α β] [LawfulDMapAPI γ α β]
-    {m : γ} {f : (a : α) → β a → Bool} {k : α} (h : k ∈ filter f m) : k ∈ m := by
+      {m : γ} {f : (a : α) → β a → Bool} {k : α} (h : k ∈ filter f m) : k ∈ m := by
     apply (mem_filter.mp h).choose
 
   theorem filter_subset {γ α β} [inst : DMapAPI γ α β] [LawfulDMapAPI γ α β]
-    {m : γ} {f : (a : α) → β a → Bool} :
+      {m : γ} {f : (a : α) → β a → Bool} :
     subset (β:=β) (filter f m) m := by
     intro k v; simp_all [dGetElem?_filter]
 
   theorem filter_keySubset {γ α β} [inst : DMapAPI γ α β] [LawfulDMapAPI γ α β]
-    {m : γ} {f : (a : α) → β a → Bool} :
+      {m : γ} {f : (a : α) → β a → Bool} :
     keySubset (β:=β) (filter f m) m := fun _ => mem_of_mem_filter
 
   theorem contains_filter {γ α β} [inst : DMapAPI γ α β] [LawfulDMapAPI γ α β]
-    {m : γ} {f : (a : α) → β a → Bool} {k : α} :
+      {m : γ} {f : (a : α) → β a → Bool} {k : α} :
     Contains.contains (filter f m) k ↔ Option.any (f k) m[k]ᵈ? := by
     simp only [LawfulContainsMem.contains_iff_mem, mem_iff_dGetElem?_eq_some, dGetElem?_filter]
     simp only [Option.filter, Option.any]; grind
 
   theorem contains_of_contains_filter {γ α β} [inst : DMapAPI γ α β] [LawfulDMapAPI γ α β]
-    {m : γ} {f : (a : α) → β a → Bool} {k : α} (h : Contains.contains (filter f m) k) : Contains.contains m k := by
+      {m : γ} {f : (a : α) → β a → Bool} {k : α} (h : Contains.contains (filter f m) k) : Contains.contains m k := by
     simp only [LawfulContainsMem.contains_iff_mem, mem_filter] at *
     apply h.choose
 
   theorem dGetElem_filter {γ α β} [inst : DMapAPI γ α β] [LawfulDMapAPI γ α β]
-    {m : γ} {f : (a : α) → β a → Bool} {k : α} {h' : k ∈ filter f m} :
-    (filter f m)[k]ᵈ'h' = m[k]ᵈ'(mem_of_mem_filter h') := by
+      {m : γ} {f : (a : α) → β a → Bool} {k : α} {h' : k ∈ filter f m} :
+      (filter f m)[k]ᵈ'h' = m[k]ᵈ'(mem_of_mem_filter h') := by
     apply (dGetElem_eq_dGetElem_iff_dGetElem?_eq_dGetElem? _ _).mpr
     have ⟨h, heq⟩ := mem_filter.mp h'
     simp [dGetElem?_filter, dGetElem?_eq_some_dGetElem h, Option.filter, heq]
 
   theorem dGetElem!_filter {γ α β} [inst : DMapAPI γ α β] [LawfulDMapAPI γ α β]
-    {m : γ} {f : (a : α) → β a → Bool} {k : α} [Inhabited (β k)] :
-    (filter f m)[k]ᵈ! = (Option.filter (f k) m[k]ᵈ?).get! := by
+      {m : γ} {f : (a : α) → β a → Bool} {k : α} [Inhabited (β k)] :
+      (filter f m)[k]ᵈ! = (Option.filter (f k) m[k]ᵈ?).get! := by
     rw [dGetElem!_eq_get!_dGetElem?, dGetElem?_filter]
 
   theorem isEmpty_filter_iff {γ α β} [inst : DMapAPI γ α β] [LawfulDMapAPI γ α β]
-    {m : γ} {f : (a : α) → β a → Bool} :
-    IsEmpty.isEmpty (filter f m) ↔ ∀ (k : α) (h : k ∈ m), f k (m[k]ᵈ'h) = false := by
+      {m : γ} {f : (a : α) → β a → Bool} :
+      IsEmpty.isEmpty (filter f m) ↔ ∀ (k : α) (h : k ∈ m), f k (m[k]ᵈ'h) = false := by
     simp [isEmpty_iff_forall_not_mem, mem_filter]
 
   theorem isEmpty_filter_eq_false_iff {γ α β} [inst : DMapAPI γ α β] [LawfulDMapAPI γ α β]
-    {m : γ} {f : (a : α) → β a → Bool} :
-    IsEmpty.isEmpty (filter f m) = false ↔ ∃ (k : α) (h : k ∈ m), f k (m[k]ᵈ'h) := by
+      {m : γ} {f : (a : α) → β a → Bool} :
+      IsEmpty.isEmpty (filter f m) = false ↔ ∃ (k : α) (h : k ∈ m), f k (m[k]ᵈ'h) := by
     rw [Bool.eq_false_iff, Ne, isEmpty_filter_iff]; simp
 
   theorem size_filter_le_size {γ α β} [inst : DMapAPI γ α β] [LawfulDMapAPI γ α β]
-    {m : γ} {f : (a : α) → β a → Bool} :
-    Size.size (filter f m) ≤ Size.size m := by
+      {m : γ} {f : (a : α) → β a → Bool} :
+      Size.size (filter f m) ≤ Size.size m := by
     apply size_le_of_keySubset
     apply filter_keySubset
 
   theorem size_filter_eq_size_iff {γ α β} [inst : DMapAPI γ α β] [LawfulDMapAPI γ α β]
-    {m : γ} {f : (a : α) → β a → Bool} :
-    Size.size (filter f m) = Size.size m ↔ ∀ (k : α) (h : k ∈ m), f k (m[k]ᵈ'h) := by
+      {m : γ} {f : (a : α) → β a → Bool} :
+      Size.size (filter f m) = Size.size m ↔ ∀ (k : α) (h : k ∈ m), f k (m[k]ᵈ'h) := by
     have hsub := filter_keySubset (m:=m) (f:=f)
     have hequiv := keyEquiv_iff_size_eq_and_keySubset (β:=β) (m₁:=filter f m) (m₂:=m)
     simp only [hsub, and_true] at hequiv
@@ -251,83 +251,83 @@ namespace LawfulDMapAPI
     grind
 
   theorem modify_congr {γ₁ γ₂ α β} [inst₁ : DMapAPI γ₁ α β] [inst₂ : DMapAPI γ₂ α β]
-    [LawfulDMapAPI γ₁ α β] [LawfulDMapAPI γ₂ α β] {m₁ : γ₁} {m₂ : γ₂}
-    (hequiv : equiv (β:=β) m₁ m₂) (k : α) (f : β k → β k) :
-    equiv (β:=β) (modify m₁ k f) (modify m₂ k f) := by
+      [LawfulDMapAPI γ₁ α β] [LawfulDMapAPI γ₂ α β] {m₁ : γ₁} {m₂ : γ₂}
+      (hequiv : equiv (β:=β) m₁ m₂) (k : α) (f : β k → β k) :
+      equiv (β:=β) (modify m₁ k f) (modify m₂ k f) := by
     rw [equiv_iff_equiv']; intro k'
     by_cases k = k'
     case pos heq => cases heq; simp only [dGetElem?_modify_self, dGetElem?_congr hequiv]
     case neg hne => simp only [dGetElem?_modify_ne hne, dGetElem?_congr hequiv]
 
   theorem mem_modify {γ α β} [inst : DMapAPI γ α β] [LawfulDMapAPI γ α β]
-    {m : γ} {k k' : α} {f : β k → β k} : k' ∈ modify m k f ↔ k' ∈ m := by
+      {m : γ} {k k' : α} {f : β k → β k} : k' ∈ modify m k f ↔ k' ∈ m := by
     simp only [mem_iff_isSome_dGetElem?]
     by_cases k = k'
     case pos heq => cases heq; rw [dGetElem?_modify_self]; simp
     case neg hne => rw [dGetElem?_modify_ne hne]
 
   theorem contains_modify {γ α β} [inst : DMapAPI γ α β] [LawfulDMapAPI γ α β]
-    {m : γ} {k k' : α} {f : β k → β k} : Contains.contains (modify m k f) k' = Contains.contains m k' := by
+      {m : γ} {k k' : α} {f : β k → β k} : Contains.contains (modify m k f) k' = Contains.contains m k' := by
     apply Bool.eq_iff_iff.mpr
     simp only [LawfulContainsMem.contains_iff_mem, mem_modify]
 
   theorem modify_keyEquiv {γ α β} [inst : DMapAPI γ α β] [LawfulDMapAPI γ α β]
-    {m : γ} {k : α} {f : β k → β k} : keyEquiv (β:=β) (modify m k f) m :=
+      {m : γ} {k : α} {f : β k → β k} : keyEquiv (β:=β) (modify m k f) m :=
     fun _ => mem_modify
 
   theorem size_modify {γ α β} [inst : DMapAPI γ α β] [LawfulDMapAPI γ α β]
-    {m : γ} {k : α} {f : β k → β k} : Size.size (modify m k f) = Size.size m := by
+      {m : γ} {k : α} {f : β k → β k} : Size.size (modify m k f) = Size.size m := by
     apply size_eq_of_keyEquiv; apply modify_keyEquiv
 
   theorem isEmpty_modify {γ α β} [inst : DMapAPI γ α β] [LawfulDMapAPI γ α β]
-    {m : γ} {k : α} {f : β k → β k} : IsEmpty.isEmpty (modify m k f) = IsEmpty.isEmpty m := by
+      {m : γ} {k : α} {f : β k → β k} : IsEmpty.isEmpty (modify m k f) = IsEmpty.isEmpty m := by
     apply Bool.eq_iff_iff.mpr
     simp only [LawfulIsEmptySize.isEmpty_iff_size_eq_zero, size_modify]
 
   theorem dGetElem_modify_self {γ α β} [inst : DMapAPI γ α β] [LawfulDMapAPI γ α β]
-    {m : γ} {k : α} {f : β k → β k} (h : k ∈ modify m k f) :
-    (DMapAPI.modify m k f)[k]ᵈ'h = f (m[k]ᵈ'(mem_modify.mp h)) := by
+      {m : γ} {k : α} {f : β k → β k} (h : k ∈ modify m k f) :
+      (DMapAPI.modify m k f)[k]ᵈ'h = f (m[k]ᵈ'(mem_modify.mp h)) := by
     rw [dGetElem_eq_iff_dGetElem?_eq_some]
     rw [dGetElem?_modify_self, dGetElem?_eq_some_dGetElem (mem_modify.mp h)]
     rfl
 
   theorem dGetElem_modify_self' {γ α β} [inst : DMapAPI γ α β] [LawfulDMapAPI γ α β]
-    {m : γ} {k : α} {f : β k → β k} (h : k ∈ m) :
-    (DMapAPI.modify m k f)[k]ᵈ'(mem_modify.mpr h) = f (m[k]ᵈ'h) :=
+      {m : γ} {k : α} {f : β k → β k} (h : k ∈ m) :
+      (DMapAPI.modify m k f)[k]ᵈ'(mem_modify.mpr h) = f (m[k]ᵈ'h) :=
     dGetElem_modify_self (mem_modify.mpr h)
 
   theorem dGetElem_modify_ne {γ α β} [inst : DMapAPI γ α β] [LawfulDMapAPI γ α β]
-    {m : γ} {k a : α} {f : β k → β k} (h : a ∈ modify m k f) (hne : k ≠ a) :
-    (DMapAPI.modify m k f)[a]ᵈ'h = m[a]ᵈ'(mem_modify.mp h) := by
+      {m : γ} {k a : α} {f : β k → β k} (h : a ∈ modify m k f) (hne : k ≠ a) :
+      (DMapAPI.modify m k f)[a]ᵈ'h = m[a]ᵈ'(mem_modify.mp h) := by
     rw [dGetElem_eq_dGetElem_iff_dGetElem?_eq_dGetElem?]
     rw [dGetElem?_modify_ne hne]
 
   theorem dGetElem_modify_ne' {γ α β} [inst : DMapAPI γ α β] [LawfulDMapAPI γ α β]
-    {m : γ} {k a : α} {f : β k → β k} (h : a ∈ m) (hne : k ≠ a) :
-    (DMapAPI.modify m k f)[a]ᵈ'(mem_modify.mpr h) = m[a]ᵈ'h :=
+      {m : γ} {k a : α} {f : β k → β k} (h : a ∈ m) (hne : k ≠ a) :
+      (DMapAPI.modify m k f)[a]ᵈ'(mem_modify.mpr h) = m[a]ᵈ'h :=
     dGetElem_modify_ne (mem_modify.mpr h) hne
 
   theorem dGetElem!_modify_self {γ α β} [inst : DMapAPI γ α β] [LawfulDMapAPI γ α β]
-    {m : γ} {k : α} [Inhabited (β k)] {f : β k → β k} : (modify m k f)[k]ᵈ! = (Option.map f m[k]ᵈ?).get! := by
+      {m : γ} {k : α} [Inhabited (β k)] {f : β k → β k} : (modify m k f)[k]ᵈ! = (Option.map f m[k]ᵈ?).get! := by
     rw [dGetElem!_eq_get!_dGetElem?, dGetElem?_modify_self]
 
   theorem dGetElem!_modify_ne {γ α β} [inst : DMapAPI γ α β] [LawfulDMapAPI γ α β]
-    {m : γ} {k k' : α} [Inhabited (β k')] {f : β k → β k} (h : k ≠ k'):
-    (modify m k f)[k']ᵈ! = m[k']ᵈ! := by
+      {m : γ} {k k' : α} [Inhabited (β k')] {f : β k → β k} (h : k ≠ k'):
+      (modify m k f)[k']ᵈ! = m[k']ᵈ! := by
     simp only [dGetElem!_eq_get!_dGetElem?, dGetElem?_modify_ne h]
 
   theorem alter_congr {γ₁ γ₂ α β} [inst₁ : DMapAPI γ₁ α β] [inst₂ : DMapAPI γ₂ α β]
-    [LawfulDMapAPI γ₁ α β] [LawfulDMapAPI γ₂ α β] {m₁ : γ₁} {m₂ : γ₂}
-    (hequiv : equiv (β:=β) m₁ m₂) (k : α) (f : Option (β k) → Option (β k)) :
-    equiv (β:=β) (alter m₁ k f) (alter m₂ k f) := by
+      [LawfulDMapAPI γ₁ α β] [LawfulDMapAPI γ₂ α β] {m₁ : γ₁} {m₂ : γ₂}
+      (hequiv : equiv (β:=β) m₁ m₂) (k : α) (f : Option (β k) → Option (β k)) :
+      equiv (β:=β) (alter m₁ k f) (alter m₂ k f) := by
     rw [equiv_iff_equiv']; intro k'
     by_cases k = k'
     case pos heq => cases heq; simp only [dGetElem?_alter_self, dGetElem?_congr hequiv]
     case neg hne => simp only [dGetElem?_alter_ne hne, dGetElem?_congr hequiv]
 
   theorem alter_none {γ α β} [inst : DMapAPI γ α β] [LawfulDMapAPI γ α β]
-    {m : γ} {k : α} {f : Option (β k) → Option (β k)}
-    (hnone : f m[k]ᵈ? = .none) : equiv (β:=β) (alter m k f) (erase (β:=β) m k) := by
+      {m : γ} {k : α} {f : Option (β k) → Option (β k)}
+      (hnone : f m[k]ᵈ? = .none) : equiv (β:=β) (alter m k f) (erase (β:=β) m k) := by
     rw [equiv_iff_equiv']; intro x
     by_cases k = x
     case pos heq =>
@@ -337,8 +337,8 @@ namespace LawfulDMapAPI
       rw [dGetElem?_alter_ne hne, dGetElem?_erase_ne hne]
 
   theorem alter_some {γ α β} [inst : DMapAPI γ α β] [LawfulDMapAPI γ α β]
-    {m : γ} {k : α} {v : β k} {f : Option (β k) → Option (β k)}
-    (hsome : f m[k]ᵈ? = .some v) : equiv (β:=β) (alter m k f) (insert m k v) := by
+      {m : γ} {k : α} {v : β k} {f : Option (β k) → Option (β k)}
+      (hsome : f m[k]ᵈ? = .some v) : equiv (β:=β) (alter m k f) (insert m k v) := by
     rw [equiv_iff_equiv']; intro x
     by_cases k = x
     case pos heq =>
@@ -348,59 +348,59 @@ namespace LawfulDMapAPI
       rw [dGetElem?_alter_ne hne, dGetElem?_insert_ne hne]
 
   theorem mem_alter_self {γ α β} [inst : DMapAPI γ α β] [LawfulDMapAPI γ α β]
-    {m : γ} {k : α} {f : Option (β k) → Option (β k)} :
-    k ∈ alter m k f ↔ (f m[k]ᵈ?).isSome := by
+      {m : γ} {k : α} {f : Option (β k) → Option (β k)} :
+      k ∈ alter m k f ↔ (f m[k]ᵈ?).isSome := by
     simp only [mem_iff_dGetElem?_eq_some, dGetElem?_alter_self]
     rw [Option.isSome_iff_exists]
 
   theorem mem_alter_ne {γ α β} [inst : DMapAPI γ α β] [LawfulDMapAPI γ α β]
-    {m : γ} {k k' : α} {f : Option (β k) → Option (β k)} (hne : k ≠ k') :
-    k' ∈ alter m k f ↔ k' ∈ m := by
+      {m : γ} {k k' : α} {f : Option (β k) → Option (β k)} (hne : k ≠ k') :
+      k' ∈ alter m k f ↔ k' ∈ m := by
     simp only [mem_iff_dGetElem?_eq_some, dGetElem?_alter_ne hne]
 
   theorem contains_alter_self {γ α β} [inst : DMapAPI γ α β] [LawfulDMapAPI γ α β]
-    {m : γ} {k : α} {f : Option (β k) → Option (β k)} :
-    Contains.contains (alter m k f) k = (f m[k]ᵈ?).isSome := by
+      {m : γ} {k : α} {f : Option (β k) → Option (β k)} :
+      Contains.contains (alter m k f) k = (f m[k]ᵈ?).isSome := by
     rw [Bool.eq_iff_iff, LawfulContainsMem.contains_iff_mem]
     apply mem_alter_self
 
   theorem contains_alter_ne {γ α β} [inst : DMapAPI γ α β] [LawfulDMapAPI γ α β]
-    {m : γ} {k k' : α} {f : Option (β k) → Option (β k)} (hne : k ≠ k') :
-    Contains.contains (alter m k f) k' = Contains.contains m k' := by
+      {m : γ} {k k' : α} {f : Option (β k) → Option (β k)} (hne : k ≠ k') :
+      Contains.contains (alter m k f) k' = Contains.contains m k' := by
     rw [Bool.eq_iff_iff]; simp only [LawfulContainsMem.contains_iff_mem]
     apply mem_alter_ne hne
 
   theorem size_alter_eq_add_one {γ α β} [inst : DMapAPI γ α β] [LawfulDMapAPI γ α β]
-    {m : γ} {k : α} {f : Option (β k) → Option (β k)}
-    (h : ¬k ∈ m) (h' : (f m[k]ᵈ?).isSome) :
-    Size.size (alter m k f) = Size.size m + 1 := by
+      {m : γ} {k : α} {f : Option (β k) → Option (β k)}
+      (h : ¬k ∈ m) (h' : (f m[k]ᵈ?).isSome) :
+      Size.size (alter m k f) = Size.size m + 1 := by
     have ⟨a, ha⟩ := Option.isSome_iff_exists.mp h'
     rw [size_congr (alter_some ha), size_insert_not_mem h]
 
   theorem size_alter_eq_self_of_mem {γ α β} [inst : DMapAPI γ α β] [LawfulDMapAPI γ α β]
-    {m : γ} {k : α} {f : Option (β k) → Option (β k)}
-    (h : k ∈ m) (h' : (f m[k]ᵈ?).isSome) :
-    Size.size (alter m k f) = Size.size m := by
+      {m : γ} {k : α} {f : Option (β k) → Option (β k)}
+      (h : k ∈ m) (h' : (f m[k]ᵈ?).isSome) :
+      Size.size (alter m k f) = Size.size m := by
     have ⟨a, ha⟩ := Option.isSome_iff_exists.mp h'
     rw [size_congr (alter_some ha), size_insert_mem h]
 
   theorem size_alter_eq_self_of_not_mem {γ α β} [inst : DMapAPI γ α β] [LawfulDMapAPI γ α β]
-    {m : γ} {k : α} {f : Option (β k) → Option (β k)}
-    (h : k ∉ m) (h' : (f m[k]ᵈ?).isNone) :
-    Size.size (alter m k f) = Size.size m := by
+      {m : γ} {k : α} {f : Option (β k) → Option (β k)}
+      (h : k ∉ m) (h' : (f m[k]ᵈ?).isNone) :
+      Size.size (alter m k f) = Size.size m := by
     rw [Option.isNone_iff_eq_none] at h'
     rw [size_congr (alter_none h'), size_erase_not_mem h]
 
   theorem size_alter_eq_sub_one {γ α β} [inst : DMapAPI γ α β] [LawfulDMapAPI γ α β]
-    {m : γ} {k : α} {f : Option (β k) → Option (β k)}
-    (h : k ∈ m) (h' : (f m[k]ᵈ?).isNone) :
-    Size.size (alter m k f) + 1 = Size.size m := by
+      {m : γ} {k : α} {f : Option (β k) → Option (β k)}
+      (h : k ∈ m) (h' : (f m[k]ᵈ?).isNone) :
+      Size.size (alter m k f) + 1 = Size.size m := by
     rw [Option.isNone_iff_eq_none] at h'
     rw [size_congr (alter_none h'), size_erase_mem h]
 
   theorem size_alter_le_size {γ α β} [inst : DMapAPI γ α β] [LawfulDMapAPI γ α β]
-    {m : γ} {k : α} {f : Option (β k) → Option (β k)} :
-    Size.size (alter m k f) ≤ Size.size m + 1 := by
+      {m : γ} {k : α} {f : Option (β k) → Option (β k)} :
+      Size.size (alter m k f) ≤ Size.size m + 1 := by
     cases h : f m[k]ᵈ?
     case none =>
       rw [size_congr (alter_none h)]
@@ -410,8 +410,8 @@ namespace LawfulDMapAPI
       apply size_insert_le
 
   theorem size_le_size_alter {γ α β} [inst : DMapAPI γ α β] [LawfulDMapAPI γ α β]
-    {m : γ} {k : α} {f : Option (β k) → Option (β k)} :
-    Size.size m ≤ Size.size (alter m k f) + 1:= by
+      {m : γ} {k : α} {f : Option (β k) → Option (β k)} :
+      Size.size m ≤ Size.size (alter m k f) + 1:= by
     cases h : f m[k]ᵈ?
     case none =>
       rw [size_congr (alter_none h)]
@@ -421,15 +421,15 @@ namespace LawfulDMapAPI
       have := le_size_insert (β:=β) (m:=m) (k:=k) (v:=v); omega
 
   theorem isEmpty_alter {γ α β} [inst : DMapAPI γ α β] [LawfulDMapAPI γ α β]
-    {m : γ} {k : α} {f : Option (β k) → Option (β k)} :
-    IsEmpty.isEmpty (alter m k f) = ((IsEmpty.isEmpty m || Size.size m == 1 && Contains.contains m k) && (f m[k]ᵈ?).isNone) := by
+      {m : γ} {k : α} {f : Option (β k) → Option (β k)} :
+      IsEmpty.isEmpty (alter m k f) = ((IsEmpty.isEmpty m || Size.size m == 1 && Contains.contains m k) && (f m[k]ᵈ?).isNone) := by
     cases h : f m[k]ᵈ?
     case none => simp [isEmpty_congr (alter_none h), isEmpty_erase]
     case some => simp [isEmpty_congr (alter_some h), isEmpty_insert_eq_false]
 
   theorem isEmpty_alter_eq_isEmpty_erase {γ α β} [inst : DMapAPI γ α β] [LawfulDMapAPI γ α β]
-    {m : γ} {k : α} {f : Option (β k) → Option (β k)} :
-    IsEmpty.isEmpty (alter m k f) = (IsEmpty.isEmpty (erase (β:=β) m k) && (f m[k]ᵈ?).isNone) := by
+      {m : γ} {k : α} {f : Option (β k) → Option (β k)} :
+      IsEmpty.isEmpty (alter m k f) = (IsEmpty.isEmpty (erase (β:=β) m k) && (f m[k]ᵈ?).isNone) := by
     rw [Bool.eq_iff_iff]
     simp only [Bool.and_eq_true, Option.isNone_iff_eq_none]
     cases h : f m[k]ᵈ?
@@ -437,23 +437,23 @@ namespace LawfulDMapAPI
     case some => rw [isEmpty_congr (alter_some h)]; simp [isEmpty_insert_eq_false]
 
   theorem dGetElem_alter_self {γ α β} [inst : DMapAPI γ α β] [LawfulDMapAPI γ α β]
-    {m : γ} {k : α} {f : Option (β k) → Option (β k)} {h : k ∈ alter m k f} :
-    (alter m k f)[k]ᵈ'h = (f m[k]ᵈ?).get (mem_alter_self.mp h) := by
+      {m : γ} {k : α} {f : Option (β k) → Option (β k)} {h : k ∈ alter m k f} :
+      (alter m k f)[k]ᵈ'h = (f m[k]ᵈ?).get (mem_alter_self.mp h) := by
     rw [dGetElem_eq_iff_dGetElem?_eq_some, dGetElem?_alter_self, Option.some_get]
 
   theorem dGetElem_alter_ne {γ α β} [inst : DMapAPI γ α β] [LawfulDMapAPI γ α β]
-    {m : γ} {k k' : α} {f : Option (β k) → Option (β k)} {h : k' ∈ alter m k f} (hne : k ≠ k') :
-    (alter m k f)[k']ᵈ'h = m[k']ᵈ'((mem_alter_ne hne).mp h) := by
+      {m : γ} {k k' : α} {f : Option (β k) → Option (β k)} {h : k' ∈ alter m k f} (hne : k ≠ k') :
+      (alter m k f)[k']ᵈ'h = m[k']ᵈ'((mem_alter_ne hne).mp h) := by
     rw [dGetElem_eq_iff_dGetElem?_eq_some, dGetElem?_alter_ne hne, dGetElem?_eq_some_dGetElem]
 
   theorem dGetElem!_alter_self {γ α β} [inst : DMapAPI γ α β] [LawfulDMapAPI γ α β]
-    {m : γ} {k : α} [Inhabited (β k)] {f : Option (β k) → Option (β k)} :
-    (alter m k f)[k]ᵈ! = (f m[k]ᵈ?).get! := by
+      {m : γ} {k : α} [Inhabited (β k)] {f : Option (β k) → Option (β k)} :
+      (alter m k f)[k]ᵈ! = (f m[k]ᵈ?).get! := by
     rw [dGetElem!_eq_get!_dGetElem?, dGetElem?_alter_self]
 
   theorem dGetElem!_alter_ne {γ α β} [inst : DMapAPI γ α β] [LawfulDMapAPI γ α β]
-    {m : γ} {k k' : α} [Inhabited (β k')] {f : Option (β k) → Option (β k)} (hne : k ≠ k') :
-    (alter m k f)[k']ᵈ! = m[k']ᵈ! := by
+      {m : γ} {k k' : α} [Inhabited (β k')] {f : Option (β k) → Option (β k)} (hne : k ≠ k') :
+      (alter m k f)[k']ᵈ! = m[k']ᵈ! := by
     simp [dGetElem!_eq_get!_dGetElem?, dGetElem?_alter_ne hne]
 
 end LawfulDMapAPI
@@ -608,7 +608,7 @@ end DMapAPI
 section MapAPI
 
 class MapAPI (γ : Type u) (α : Type v) (β : Type w) extends
-  MapLike γ α β, IsEmpty γ, Contains γ α where
+    MapLike γ α β, IsEmpty γ, Contains γ α where
   insertIfNew : γ → α → β → γ
   containsThenInsert : γ → α → β → Bool × γ
   containsThenInsertIfNew : γ → α → β → Bool × γ
@@ -646,7 +646,7 @@ def MapAPI_DMapAPI_inv {γ α β} {inst : MapAPI γ α β} :
 open MapAPI MapLike
 
 class LawfulMapAPI (γ : Type u) (α : Type v) (β : Type w) [inst : MapAPI γ α β]
-  extends LawfulMapLike γ α β, LawfulIsEmptySize γ, LawfulContainsMem γ α where
+    extends LawfulMapLike γ α β, LawfulIsEmptySize γ, LawfulContainsMem γ α where
   getElem?_insertIfNew_self {m : γ} {k : α} {v : β} (h : k ∉ m) :
     (insertIfNew m k v)[k]? = .some v
   getElem?_insertIfNew_ne {m : γ} {k a : α} {v : β} (h : k ≠ a ∨ k ∈ m) :
@@ -668,8 +668,8 @@ class LawfulMapAPI (γ : Type u) (α : Type v) (β : Type w) [inst : MapAPI γ �
     (alter m k f)[k']? = m[k']?
 
 def LawfulMapAPI_of_LawfulDMapAPI {γ α β} [inst : MapAPI γ α β]
-  [instL : LawfulDMapAPI (inst:=DMapAPI_of_MapAPI inst) γ α (fun _ => β)] :
-  LawfulMapAPI γ α β where
+    [instL : LawfulDMapAPI (inst:=DMapAPI_of_MapAPI inst) γ α (fun _ => β)] :
+    LawfulMapAPI γ α β where
   toLawfulMapLike := LawfulMapLike_of_LawfulDMapLike (inst:=inst.toMapLike) (instL:=instL.toLawfulDMapLike)
   isEmpty_iff_size_eq_zero := instL.isEmpty_iff_size_eq_zero
   contains_iff_mem := instL.contains_iff_mem
@@ -688,13 +688,13 @@ def LawfulMapAPI_of_LawfulDMapAPI {γ α β} [inst : MapAPI γ α β]
   getElem?_alter_ne := instL.dGetElem?_alter_ne
 
 theorem LawfulMapAPI_of_LawfulDMapAPI' {γ α β} [inst : DMapAPI γ α (fun _ => β)]
-  [instL : LawfulDMapAPI γ α (fun _ => β)] :
-  LawfulMapAPI (inst:=MapAPI_of_DMapAPI inst) γ α β :=
+    [instL : LawfulDMapAPI γ α (fun _ => β)] :
+    LawfulMapAPI (inst:=MapAPI_of_DMapAPI inst) γ α β :=
   LawfulMapAPI_of_LawfulDMapAPI (inst:=MapAPI_of_DMapAPI inst)
 
 def LawfulDMapAPI_of_LawfulMapAPI {γ α β} [inst : DMapAPI γ α (fun _ => β)]
-  [instL : LawfulMapAPI (inst:=MapAPI_of_DMapAPI inst) γ α β] :
-  LawfulDMapAPI γ α (fun _ => β) where
+    [instL : LawfulMapAPI (inst:=MapAPI_of_DMapAPI inst) γ α β] :
+    LawfulDMapAPI γ α (fun _ => β) where
   toLawfulDMapLike := LawfulDMapLike_of_LawfulMapLike (inst:=inst.toDMapLike) (instL:=instL.toLawfulMapLike)
   isEmpty_iff_size_eq_zero := instL.isEmpty_iff_size_eq_zero
   contains_iff_mem := instL.contains_iff_mem
@@ -712,9 +712,8 @@ def LawfulDMapAPI_of_LawfulMapAPI {γ α β} [inst : DMapAPI γ α (fun _ => β)
   dGetElem?_alter_self := instL.getElem?_alter_self
   dGetElem?_alter_ne := instL.getElem?_alter_ne
 
-local instance LawfulDMapAPI_of_LawfulMapAPI' {γ α β} [inst : MapAPI γ α β]
-  [instL : LawfulMapAPI γ α β] :
-  LawfulDMapAPI (inst:=DMapAPI_of_MapAPI inst) γ α (fun _ => β) :=
+local instance LawfulDMapAPI_of_LawfulMapAPI' {γ α β} [inst : MapAPI γ α β] [instL : LawfulMapAPI γ α β] :
+    LawfulDMapAPI (inst:=DMapAPI_of_MapAPI inst) γ α (fun _ => β) :=
   LawfulDMapAPI_of_LawfulMapAPI (inst:=DMapAPI_of_MapAPI inst)
 
 namespace LawfulMapAPI
@@ -722,317 +721,318 @@ namespace LawfulMapAPI
   open LawfulMapLike
 
   theorem isEmpty_congr {γ₁ γ₂ α β} [inst₁ : MapAPI γ₁ α β] [inst₂ : MapAPI γ₂ α β]
-    [LawfulMapAPI γ₁ α β] [LawfulMapAPI γ₂ α β] {m₁ : γ₁} {m₂ : γ₂}
-    (hequiv : equiv (α:=α) (β:=β) m₁ m₂) : IsEmpty.isEmpty m₁ = IsEmpty.isEmpty m₂ :=
+      [LawfulMapAPI γ₁ α β] [LawfulMapAPI γ₂ α β] {m₁ : γ₁} {m₂ : γ₂}
+      (hequiv : equiv (α:=α) (β:=β) m₁ m₂) : IsEmpty.isEmpty m₁ = IsEmpty.isEmpty m₂ :=
     LawfulDMapAPI.isEmpty_congr (inst₁:=DMapAPI_of_MapAPI inst₁) (inst₂:=DMapAPI_of_MapAPI inst₂) hequiv
 
   theorem isEmpty_erase {γ α β} [inst : MapAPI γ α β] [LawfulMapAPI γ α β]
-    {m : γ} {k : α} : IsEmpty.isEmpty (erase (β:=β) m k) = (IsEmpty.isEmpty m || (Size.size m == 1 && Contains.contains m k)) :=
+      {m : γ} {k : α} : IsEmpty.isEmpty (erase (β:=β) m k) = (IsEmpty.isEmpty m || (Size.size m == 1 && Contains.contains m k)) :=
     LawfulDMapAPI.isEmpty_erase (inst:=DMapAPI_of_MapAPI inst)
 
   theorem isEmpty_insert_eq_false {γ α β} [inst : MapAPI γ α β] [LawfulMapAPI γ α β]
-    {m : γ} {k : α} {v : β} : IsEmpty.isEmpty (insert m k v) = false :=
+      {m : γ} {k : α} {v : β} : IsEmpty.isEmpty (insert m k v) = false :=
     LawfulDMapAPI.isEmpty_insert_eq_false (inst:=DMapAPI_of_MapAPI inst)
 
   theorem contains_congr {γ₁ γ₂ α β} [inst₁ : MapAPI γ₁ α β] [inst₂ : MapAPI γ₂ α β]
-    [LawfulMapAPI γ₁ α β] [LawfulMapAPI γ₂ α β] {m₁ : γ₁} {m₂ : γ₂}
-    (hequiv : equiv (α:=α) (β:=β) m₁ m₂) (k : α) : Contains.contains m₁ k = Contains.contains m₂ k :=
+      [LawfulMapAPI γ₁ α β] [LawfulMapAPI γ₂ α β] {m₁ : γ₁} {m₂ : γ₂}
+      (hequiv : equiv (α:=α) (β:=β) m₁ m₂) (k : α) : Contains.contains m₁ k = Contains.contains m₂ k :=
     LawfulDMapAPI.contains_congr (inst₁:=DMapAPI_of_MapAPI inst₁) (inst₂:=DMapAPI_of_MapAPI inst₂) hequiv _
 
   theorem not_contains_iff_not_mem {γ α β} [inst : MapAPI γ α β] [LawfulMapAPI γ α β]
-    {m : γ} {k : α} : Contains.contains m k = false ↔ k ∉ m :=
+      {m : γ} {k : α} : Contains.contains m k = false ↔ k ∉ m :=
     LawfulDMapAPI.not_contains_iff_not_mem (inst:=DMapAPI_of_MapAPI inst)
 
   theorem isEmpty_iff_forall_not_mem {γ α β} [inst : MapAPI γ α β] [LawfulMapAPI γ α β]
-    {m : γ} : IsEmpty.isEmpty m ↔ ∀ (x : α), x ∉ m :=
+      {m : γ} : IsEmpty.isEmpty m ↔ ∀ (x : α), x ∉ m :=
     LawfulDMapAPI.isEmpty_iff_forall_not_mem (inst:=DMapAPI_of_MapAPI inst)
 
   theorem insertIfNew_equiv_of_mem {γ α β} [inst : MapAPI γ α β] [LawfulMapAPI γ α β]
-    {m : γ} {k : α} {v : β} (h : k ∈ m) : equiv (α:=α) (β:=β) (insertIfNew m k v) m :=
+      {m : γ} {k : α} {v : β} (h : k ∈ m) : equiv (α:=α) (β:=β) (insertIfNew m k v) m :=
     LawfulDMapAPI.insertIfNew_equiv_of_mem (inst:=DMapAPI_of_MapAPI inst) h
 
   theorem insertIfNew_equiv_of_not_mem {γ α β} [inst : MapAPI γ α β] [LawfulMapAPI γ α β]
-    {m : γ} {k : α} {v : β} (h : k ∉ m) : equiv (α:=α) (β:=β) (insertIfNew m k v) (insert m k v) :=
+      {m : γ} {k : α} {v : β} (h : k ∉ m) : equiv (α:=α) (β:=β) (insertIfNew m k v) (insert m k v) :=
     LawfulDMapAPI.insertIfNew_equiv_of_not_mem (inst:=DMapAPI_of_MapAPI inst) h
 
   theorem insertIfNew_equiv {γ α β} [inst : MapAPI γ α β] [LawfulMapAPI γ α β]
-    {m : γ} {k : α} {v : β} : equiv (α:=α) (β:=β) (insertIfNew m k v) (if Contains.contains m k then m else insert m k v) :=
+      {m : γ} {k : α} {v : β} : equiv (α:=α) (β:=β) (insertIfNew m k v) (if Contains.contains m k then m else insert m k v) :=
     LawfulDMapAPI.insertIfNew_equiv (inst:=DMapAPI_of_MapAPI inst)
 
   theorem insertIfNew_congr {γ₁ γ₂ α β} [inst₁ : MapAPI γ₁ α β] [inst₂ : MapAPI γ₂ α β]
-    [LawfulMapAPI γ₁ α β] [LawfulMapAPI γ₂ α β] {m₁ : γ₁} {m₂ : γ₂}
-    (hequiv : equiv (α:=α) (β:=β) m₁ m₂) (k : α) (v : β) :
-    equiv (α:=α) (β:=β) (insertIfNew m₁ k v) (insertIfNew m₂ k v) :=
+      [LawfulMapAPI γ₁ α β] [LawfulMapAPI γ₂ α β] {m₁ : γ₁} {m₂ : γ₂}
+      (hequiv : equiv (α:=α) (β:=β) m₁ m₂) (k : α) (v : β) :
+      equiv (α:=α) (β:=β) (insertIfNew m₁ k v) (insertIfNew m₂ k v) :=
     LawfulDMapAPI.insertIfNew_congr (inst₁:=DMapAPI_of_MapAPI inst₁) (inst₂:=DMapAPI_of_MapAPI inst₂) hequiv _ _
 
   theorem size_insertIfNew_mem {γ α β} [inst : MapAPI γ α β] [LawfulMapAPI γ α β]
-    {m : γ} {k : α} {v : β} (h : k ∈ m) : Size.size (insertIfNew m k v) = Size.size m :=
+      {m : γ} {k : α} {v : β} (h : k ∈ m) : Size.size (insertIfNew m k v) = Size.size m :=
     LawfulDMapAPI.size_insertIfNew_mem (inst:=DMapAPI_of_MapAPI inst) h
 
   theorem size_insertIfNew_not_mem {γ α β} [inst : MapAPI γ α β] [LawfulMapAPI γ α β]
-    {m : γ} {k : α} {v : β} (h : k ∉ m) : Size.size (insertIfNew m k v) = Size.size m + 1 :=
+      {m : γ} {k : α} {v : β} (h : k ∉ m) : Size.size (insertIfNew m k v) = Size.size m + 1 :=
     LawfulDMapAPI.size_insertIfNew_not_mem (inst:=DMapAPI_of_MapAPI inst) h
 
   theorem size_insertIfNew {γ α β} [inst : MapAPI γ α β] [LawfulMapAPI γ α β]
-    {m : γ} {k : α} [Decidable (k ∈ m)] {v : β} : Size.size (insertIfNew m k v) = if k ∈ m then Size.size m else Size.size m + 1 :=
+      {m : γ} {k : α} [Decidable (k ∈ m)] {v : β} : Size.size (insertIfNew m k v) = if k ∈ m then Size.size m else Size.size m + 1 :=
     LawfulDMapAPI.size_insertIfNew (inst:=DMapAPI_of_MapAPI inst)
 
   theorem mem_insertIfNew' {γ α β} [inst : MapAPI γ α β] [LawfulMapAPI γ α β]
-    {m : γ} {k a : α} {v : β} : a ∈ MapAPI.insertIfNew m k v ↔ k = a ∨ a ∈ m :=
+      {m : γ} {k a : α} {v : β} : a ∈ MapAPI.insertIfNew m k v ↔ k = a ∨ a ∈ m :=
     LawfulDMapAPI.mem_insertIfNew' (inst:=DMapAPI_of_MapAPI inst)
 
   theorem mem_insertIfNew {γ α β} [BEq α] [LawfulBEq α] [inst : MapAPI γ α β] [LawfulMapAPI γ α β]
-    {m : γ} {k a : α} {v : β} : a ∈ MapAPI.insertIfNew m k v ↔ k == a ∨ a ∈ m :=
+      {m : γ} {k a : α} {v : β} : a ∈ MapAPI.insertIfNew m k v ↔ k == a ∨ a ∈ m :=
     LawfulDMapAPI.mem_insertIfNew (inst:=DMapAPI_of_MapAPI inst)
 
   theorem mem_of_mem_insertIfNew' {γ α β} [inst : MapAPI γ α β] [LawfulMapAPI γ α β] {m : γ} {k a : α} {v : β} :
-    a ∈ insertIfNew m k v → k ≠ a ∨ k ∈ m → a ∈ m :=
+      a ∈ insertIfNew m k v → k ≠ a ∨ k ∈ m → a ∈ m :=
     LawfulDMapAPI.mem_of_mem_insertIfNew' (inst:=DMapAPI_of_MapAPI inst)
 
   theorem contains_insertIfNew {γ α β} [inst : MapAPI γ α β] [LawfulMapAPI γ α β]
-    {m : γ} {k a : α} {v : β} : Contains.contains (MapAPI.insertIfNew m k v) a ↔ k = a ∨ a ∈ m :=
+      {m : γ} {k a : α} {v : β} : Contains.contains (MapAPI.insertIfNew m k v) a ↔ k = a ∨ a ∈ m :=
     LawfulDMapAPI.contains_insertIfNew (inst:=DMapAPI_of_MapAPI inst)
 
   theorem getElem_insertIfNew_ne {γ α β} [inst : MapAPI γ α β] [LawfulMapAPI γ α β]
-    {m : γ} {k a : α} {v : β} {h₁ : a ∈ insertIfNew m k v} {h₂ : k ≠ a ∨ k ∈ m} :
-    (insertIfNew m k v)[a]'h₁ = m[a]'(mem_of_mem_insertIfNew' h₁ h₂) :=
+      {m : γ} {k a : α} {v : β} {h₁ : a ∈ insertIfNew m k v} {h₂ : k ≠ a ∨ k ∈ m} :
+      (insertIfNew m k v)[a]'h₁ = m[a]'(mem_of_mem_insertIfNew' h₁ h₂) :=
     LawfulDMapAPI.dGetElem_insertIfNew_ne (inst:=DMapAPI_of_MapAPI inst) (h₁:=h₁) (h₂:=h₂)
 
   theorem getElem_insertIfNew_ne' {γ α β} [inst : MapAPI γ α β] [LawfulMapAPI γ α β]
-    {m : γ} {k a : α} {v : β} {h : a ∈ m} :
-    (insertIfNew m k v)[a]'(mem_insertIfNew'.mpr (Or.inr h)) = m[a]'h :=
+      {m : γ} {k a : α} {v : β} {h : a ∈ m} :
+      (insertIfNew m k v)[a]'(mem_insertIfNew'.mpr (Or.inr h)) = m[a]'h :=
     LawfulDMapAPI.dGetElem_insertIfNew_ne' (inst:=DMapAPI_of_MapAPI inst)
 
   theorem getElem_insertIfNew_self {γ α β} [inst : MapAPI γ α β] [LawfulMapAPI γ α β]
-    {m : γ} {k: α} {v : β} {h : k ∉ m} :
-    (insertIfNew m k v)[k]'(by simp [mem_insertIfNew']) = v :=
+      {m : γ} {k: α} {v : β} {h : k ∉ m} :
+      (insertIfNew m k v)[k]'(by simp [mem_insertIfNew']) = v :=
     LawfulDMapAPI.dGetElem_insertIfNew_self (inst:=DMapAPI_of_MapAPI inst) (h:=h)
 
   theorem getElem!_insertIfNew_ne {γ α β} [inst : MapAPI γ α β] [LawfulMapAPI γ α β]
-    {m : γ} {k a : α} [Inhabited β] {v : β} {h : k ≠ a ∨ k ∈ m} :
-    (insertIfNew m k v)[a]! = m[a]! :=
+      {m : γ} {k a : α} [Inhabited β] {v : β} {h : k ≠ a ∨ k ∈ m} :
+      (insertIfNew m k v)[a]! = m[a]! :=
     LawfulDMapAPI.dGetElem!_insertIfNew_ne (inst:=DMapAPI_of_MapAPI inst) (h:=h)
 
   theorem getElem!_insertIfNew_self {γ α β} [inst : MapAPI γ α β] [LawfulMapAPI γ α β]
-    {m : γ} {k : α} [Inhabited β] {v : β} {h : k ∉ m} :
-    (insertIfNew m k v)[k]! = v :=
+      {m : γ} {k : α} [Inhabited β] {v : β} {h : k ∉ m} :
+      (insertIfNew m k v)[k]! = v :=
     LawfulDMapAPI.dGetElem!_insertIfNew_self (inst:=DMapAPI_of_MapAPI inst) (h:=h)
 
   theorem filter_congr {γ₁ γ₂ α β} [inst₁ : MapAPI γ₁ α β] [inst₂ : MapAPI γ₂ α β]
-    [LawfulMapAPI γ₁ α β] [LawfulMapAPI γ₂ α β] {m₁ : γ₁} {m₂ : γ₂}
-    (hequiv : equiv (α:=α) (β:=β) m₁ m₂) (f : α → β → Bool) :
-    equiv (α:=α) (β:=β) (filter f m₁) (filter f m₂) :=
+      [LawfulMapAPI γ₁ α β] [LawfulMapAPI γ₂ α β] {m₁ : γ₁} {m₂ : γ₂}
+      (hequiv : equiv (α:=α) (β:=β) m₁ m₂) (f : α → β → Bool) :
+      equiv (α:=α) (β:=β) (filter f m₁) (filter f m₂) :=
     LawfulDMapAPI.filter_congr (inst₁:=DMapAPI_of_MapAPI inst₁) (inst₂:=DMapAPI_of_MapAPI inst₂) hequiv _
 
   theorem mem_filter {γ α β} [inst : MapAPI γ α β] [LawfulMapAPI γ α β]
-    {m : γ} {f : α → β → Bool} {k : α} :
-    k ∈ filter f m ↔ ∃ h, f k (m[k]'h) = true :=
+      {m : γ} {f : α → β → Bool} {k : α} :
+      k ∈ filter f m ↔ ∃ h, f k (m[k]'h) = true :=
     LawfulDMapAPI.mem_filter (inst:=DMapAPI_of_MapAPI inst)
 
   theorem mem_of_mem_filter {γ α β} [inst : MapAPI γ α β] [LawfulMapAPI γ α β]
-    {m : γ} {f : α → β → Bool} {k : α} (h : k ∈ filter f m) : k ∈ m :=
+      {m : γ} {f : α → β → Bool} {k : α} (h : k ∈ filter f m) : k ∈ m :=
     LawfulDMapAPI.mem_of_mem_filter (inst:=DMapAPI_of_MapAPI inst) h
 
   theorem filter_subset {γ α β} [inst : MapAPI γ α β] [LawfulMapAPI γ α β]
-    {m : γ} {f : α → β → Bool} : subset (α:=α) (β:=β) (filter f m) m :=
+      {m : γ} {f : α → β → Bool} : subset (α:=α) (β:=β) (filter f m) m :=
     LawfulDMapAPI.filter_subset (inst:=DMapAPI_of_MapAPI inst)
 
   theorem filter_keySubset {γ α β} [inst : MapAPI γ α β] [LawfulMapAPI γ α β]
-    {m : γ} {f : α → β → Bool} : keySubset (α:=α) (β:=β) (filter f m) m :=
+      {m : γ} {f : α → β → Bool} : keySubset (α:=α) (β:=β) (filter f m) m :=
     fun _ => mem_of_mem_filter
 
   theorem contains_filter {γ α β} [inst : MapAPI γ α β] [LawfulMapAPI γ α β]
-    {m : γ} {f : α → β → Bool} {k : α} :
-    Contains.contains (filter f m) k ↔ Option.any (f k) m[k]? :=
+      {m : γ} {f : α → β → Bool} {k : α} :
+      Contains.contains (filter f m) k ↔ Option.any (f k) m[k]? :=
     LawfulDMapAPI.contains_filter (inst:=DMapAPI_of_MapAPI inst)
 
   theorem contains_of_contains_filter {γ α β} [inst : MapAPI γ α β] [LawfulMapAPI γ α β]
-    {m : γ} {f : α → β → Bool} {k : α} (h : Contains.contains (filter f m) k) : Contains.contains m k :=
+      {m : γ} {f : α → β → Bool} {k : α} (h : Contains.contains (filter f m) k) : Contains.contains m k :=
     LawfulDMapAPI.contains_of_contains_filter (inst:=DMapAPI_of_MapAPI inst) h
 
+  -- **TODO: Rendering error**
   theorem getElem_filter {γ α β} [inst : MapAPI γ α β] [LawfulMapAPI γ α β]
-    {m : γ} {f : α → β → Bool} {k : α} {h' : k ∈ filter f m} :
-    (filter f m)[k]'h' = m[k]'(mem_of_mem_filter h') :=
+      {m : γ} {f : α → β → Bool} {k : α} {h' : k ∈ filter f m} :
+      (filter f m)[k]'h' = m[k]'(mem_of_mem_filter h') :=
     LawfulDMapAPI.dGetElem_filter (inst:=DMapAPI_of_MapAPI inst)
 
   theorem getElem!_filter {γ α β} [inst : MapAPI γ α β] [LawfulMapAPI γ α β]
-    {m : γ} {f : α → β → Bool} {k : α} [Inhabited β] :
-    (filter f m)[k]! = (Option.filter (f k) m[k]?).get! :=
+      {m : γ} {f : α → β → Bool} {k : α} [Inhabited β] :
+      (filter f m)[k]! = (Option.filter (f k) m[k]?).get! :=
     LawfulDMapAPI.dGetElem!_filter (inst:=DMapAPI_of_MapAPI inst)
 
   theorem isEmpty_filter_iff {γ α β} [inst : MapAPI γ α β] [LawfulMapAPI γ α β]
-    {m : γ} {f : α → β → Bool} :
+      {m : γ} {f : α → β → Bool} :
     IsEmpty.isEmpty (filter f m) ↔ ∀ (k : α) (h : k ∈ m), f k (m[k]'h) = false :=
     LawfulDMapAPI.isEmpty_filter_iff (inst:=DMapAPI_of_MapAPI inst)
 
   theorem isEmpty_filter_eq_false_iff {γ α β} [inst : MapAPI γ α β] [LawfulMapAPI γ α β]
-    {m : γ} {f : α → β → Bool} :
+      {m : γ} {f : α → β → Bool} :
     IsEmpty.isEmpty (filter f m) = false ↔ ∃ (k : α) (h : k ∈ m), f k (m[k]'h) :=
     LawfulDMapAPI.isEmpty_filter_eq_false_iff (inst:=DMapAPI_of_MapAPI inst)
 
   theorem size_filter_le_size {γ α β} [inst : MapAPI γ α β] [LawfulMapAPI γ α β]
-    {m : γ} {f : α → β → Bool} :
+      {m : γ} {f : α → β → Bool} :
     Size.size (filter f m) ≤ Size.size m :=
     LawfulDMapAPI.size_filter_le_size (inst:=DMapAPI_of_MapAPI inst)
 
   theorem size_filter_eq_size_iff {γ α β} [inst : MapAPI γ α β] [LawfulMapAPI γ α β]
-    {m : γ} {f : α → β → Bool} :
+      {m : γ} {f : α → β → Bool} :
     Size.size (filter f m) = Size.size m ↔ ∀ (k : α) (h : k ∈ m), f k (m[k]'h) :=
     LawfulDMapAPI.size_filter_eq_size_iff (inst:=DMapAPI_of_MapAPI inst)
 
   theorem modify_congr {γ₁ γ₂ α β} [inst₁ : MapAPI γ₁ α β] [inst₂ : MapAPI γ₂ α β]
-    [LawfulMapAPI γ₁ α β] [LawfulMapAPI γ₂ α β] {m₁ : γ₁} {m₂ : γ₂}
-    (hequiv : equiv (α:=α) (β:=β) m₁ m₂) (k : α) (f : β → β) :
+      [LawfulMapAPI γ₁ α β] [LawfulMapAPI γ₂ α β] {m₁ : γ₁} {m₂ : γ₂}
+      (hequiv : equiv (α:=α) (β:=β) m₁ m₂) (k : α) (f : β → β) :
     equiv (α:=α) (β:=β) (modify m₁ k f) (modify m₂ k f) :=
     LawfulDMapAPI.modify_congr (inst₁:=DMapAPI_of_MapAPI inst₁) (inst₂:=DMapAPI_of_MapAPI inst₂) hequiv _ _
 
   theorem mem_modify {γ α β} [inst : MapAPI γ α β] [LawfulMapAPI γ α β]
-    {m : γ} {k k' : α} {f : β → β} : k' ∈ modify m k f ↔ k' ∈ m :=
+      {m : γ} {k k' : α} {f : β → β} : k' ∈ modify m k f ↔ k' ∈ m :=
     LawfulDMapAPI.mem_modify (inst:=DMapAPI_of_MapAPI inst)
 
   theorem contains_modify {γ α β} [inst : MapAPI γ α β] [LawfulMapAPI γ α β]
-    {m : γ} {k k' : α} {f : β → β} : Contains.contains (modify m k f) k' = Contains.contains m k' :=
+      {m : γ} {k k' : α} {f : β → β} : Contains.contains (modify m k f) k' = Contains.contains m k' :=
     LawfulDMapAPI.contains_modify (inst:=DMapAPI_of_MapAPI inst)
 
   theorem modify_keyEquiv {γ α β} [inst : MapAPI γ α β] [LawfulMapAPI γ α β]
-    {m : γ} {k : α} {f : β → β} : keyEquiv (α:=α) (β:=β) (modify m k f) m :=
+      {m : γ} {k : α} {f : β → β} : keyEquiv (α:=α) (β:=β) (modify m k f) m :=
     fun _ => mem_modify
 
   theorem size_modify {γ α β} [inst : MapAPI γ α β] [LawfulMapAPI γ α β]
-    {m : γ} {k : α} {f : β → β} : Size.size (modify m k f) = Size.size m :=
+      {m : γ} {k : α} {f : β → β} : Size.size (modify m k f) = Size.size m :=
     LawfulDMapAPI.size_modify (inst:=DMapAPI_of_MapAPI inst)
 
   theorem isEmpty_modify {γ α β} [inst : MapAPI γ α β] [LawfulMapAPI γ α β]
-    {m : γ} {k : α} {f : β → β} : IsEmpty.isEmpty (modify m k f) = IsEmpty.isEmpty m :=
+      {m : γ} {k : α} {f : β → β} : IsEmpty.isEmpty (modify m k f) = IsEmpty.isEmpty m :=
     LawfulDMapAPI.isEmpty_modify (inst:=DMapAPI_of_MapAPI inst)
 
   theorem getElem_modify_self {γ α β} [inst : MapAPI γ α β] [LawfulMapAPI γ α β]
-    {m : γ} {k : α} {f : β → β} (h : k ∈ modify m k f) :
-    (MapAPI.modify m k f)[k]'h = f (m[k]'(mem_modify.mp h)) :=
+      {m : γ} {k : α} {f : β → β} (h : k ∈ modify m k f) :
+      (MapAPI.modify m k f)[k]'h = f (m[k]'(mem_modify.mp h)) :=
     LawfulDMapAPI.dGetElem_modify_self (inst:=DMapAPI_of_MapAPI inst) h
 
   theorem getElem_modify_self' {γ α β} [inst : MapAPI γ α β] [LawfulMapAPI γ α β]
-    {m : γ} {k : α} {f : β → β} (h : k ∈ m) :
-    (MapAPI.modify m k f)[k]'(mem_modify.mpr h) = f (m[k]'h) :=
+      {m : γ} {k : α} {f : β → β} (h : k ∈ m) :
+      (MapAPI.modify m k f)[k]'(mem_modify.mpr h) = f (m[k]'h) :=
     LawfulDMapAPI.dGetElem_modify_self' (inst:=DMapAPI_of_MapAPI inst) h
 
   theorem getElem_modify_ne {γ α β} [inst : MapAPI γ α β] [LawfulMapAPI γ α β]
-    {m : γ} {k a : α} {f : β → β} (h : a ∈ modify m k f) (hne : k ≠ a) :
-    (MapAPI.modify m k f)[a]'h = m[a]'(mem_modify.mp h) :=
+      {m : γ} {k a : α} {f : β → β} (h : a ∈ modify m k f) (hne : k ≠ a) :
+      (MapAPI.modify m k f)[a]'h = m[a]'(mem_modify.mp h) :=
     LawfulDMapAPI.dGetElem_modify_ne (inst:=DMapAPI_of_MapAPI inst) h hne
 
   theorem getElem_modify_ne' {γ α β} [inst : MapAPI γ α β] [LawfulMapAPI γ α β]
-    {m : γ} {k a : α} {f : β → β} (h : a ∈ m) (hne : k ≠ a) :
-    (MapAPI.modify m k f)[a]'(mem_modify.mpr h) = m[a]'h :=
+      {m : γ} {k a : α} {f : β → β} (h : a ∈ m) (hne : k ≠ a) :
+      (MapAPI.modify m k f)[a]'(mem_modify.mpr h) = m[a]'h :=
     getElem_modify_ne (mem_modify.mpr h) hne
 
   theorem getElem!_modify_self {γ α β} [inst : MapAPI γ α β] [LawfulMapAPI γ α β]
-    {m : γ} {k : α} [Inhabited β] {f : β → β} : (modify m k f)[k]! = (Option.map f m[k]?).get! :=
+      {m : γ} {k : α} [Inhabited β] {f : β → β} : (modify m k f)[k]! = (Option.map f m[k]?).get! :=
     LawfulDMapAPI.dGetElem!_modify_self (inst:=DMapAPI_of_MapAPI inst)
 
   theorem getElem!_modify_ne {γ α β} [inst : MapAPI γ α β] [LawfulMapAPI γ α β]
-    {m : γ} {k k' : α} [Inhabited β] {f : β → β} (h : k ≠ k'):
-    (modify m k f)[k']! = m[k']! :=
+      {m : γ} {k k' : α} [Inhabited β] {f : β → β} (h : k ≠ k'):
+      (modify m k f)[k']! = m[k']! :=
     LawfulDMapAPI.dGetElem!_modify_ne (inst:=DMapAPI_of_MapAPI inst) h
 
   theorem alter_congr {γ₁ γ₂ α β} [inst₁ : MapAPI γ₁ α β] [inst₂ : MapAPI γ₂ α β]
-    [LawfulMapAPI γ₁ α β] [LawfulMapAPI γ₂ α β] {m₁ : γ₁} {m₂ : γ₂}
-    (hequiv : equiv (α:=α) (β:=β) m₁ m₂) (k : α) (f : Option β → Option β) :
-    equiv (α:=α) (β:=β) (alter m₁ k f) (alter m₂ k f) :=
+      [LawfulMapAPI γ₁ α β] [LawfulMapAPI γ₂ α β] {m₁ : γ₁} {m₂ : γ₂}
+      (hequiv : equiv (α:=α) (β:=β) m₁ m₂) (k : α) (f : Option β → Option β) :
+      equiv (α:=α) (β:=β) (alter m₁ k f) (alter m₂ k f) :=
     LawfulDMapAPI.alter_congr (inst₁:=DMapAPI_of_MapAPI inst₁) (inst₂:=DMapAPI_of_MapAPI inst₂) hequiv _ _
 
   theorem alter_none {γ α β} [inst : MapAPI γ α β] [LawfulMapAPI γ α β]
-    {m : γ} {k : α} {f : Option β → Option β}
-    (hnone : f m[k]? = .none) : equiv (α:=α) (β:=β) (alter m k f) (erase (β:=β) m k) :=
+      {m : γ} {k : α} {f : Option β → Option β}
+      (hnone : f m[k]? = .none) : equiv (α:=α) (β:=β) (alter m k f) (erase (β:=β) m k) :=
     LawfulDMapAPI.alter_none (inst:=DMapAPI_of_MapAPI inst) hnone
 
   theorem alter_some {γ α β} [inst : MapAPI γ α β] [LawfulMapAPI γ α β]
-    {m : γ} {k : α} {v : β} {f : Option β → Option β}
-    (hsome : f m[k]? = .some v) : equiv (α:=α) (β:=β) (alter m k f) (insert m k v) :=
+      {m : γ} {k : α} {v : β} {f : Option β → Option β}
+      (hsome : f m[k]? = .some v) : equiv (α:=α) (β:=β) (alter m k f) (insert m k v) :=
     LawfulDMapAPI.alter_some (inst:=DMapAPI_of_MapAPI inst) hsome
 
   theorem mem_alter_self {γ α β} [inst : MapAPI γ α β] [LawfulMapAPI γ α β]
-    {m : γ} {k : α} {f : Option β → Option β} :
-    k ∈ alter m k f ↔ (f m[k]?).isSome :=
+      {m : γ} {k : α} {f : Option β → Option β} :
+      k ∈ alter m k f ↔ (f m[k]?).isSome :=
     LawfulDMapAPI.mem_alter_self (inst:=DMapAPI_of_MapAPI inst)
 
   theorem mem_alter_ne {γ α β} [inst : MapAPI γ α β] [LawfulMapAPI γ α β]
-    {m : γ} {k k' : α} {f : Option β → Option β} (hne : k ≠ k') :
-    k' ∈ alter m k f ↔ k' ∈ m :=
+      {m : γ} {k k' : α} {f : Option β → Option β} (hne : k ≠ k') :
+      k' ∈ alter m k f ↔ k' ∈ m :=
     LawfulDMapAPI.mem_alter_ne (inst:=DMapAPI_of_MapAPI inst) hne
 
   theorem contains_alter_self {γ α β} [inst : MapAPI γ α β] [LawfulMapAPI γ α β]
-    {m : γ} {k : α} {f : Option β → Option β} :
-    Contains.contains (alter m k f) k = (f m[k]?).isSome :=
+      {m : γ} {k : α} {f : Option β → Option β} :
+      Contains.contains (alter m k f) k = (f m[k]?).isSome :=
     LawfulDMapAPI.contains_alter_self (inst:=DMapAPI_of_MapAPI inst)
 
   theorem contains_alter_ne {γ α β} [inst : MapAPI γ α β] [LawfulMapAPI γ α β]
-    {m : γ} {k k' : α} {f : Option β → Option β} (hne : k ≠ k') :
-    Contains.contains (alter m k f) k' = Contains.contains m k' :=
+      {m : γ} {k k' : α} {f : Option β → Option β} (hne : k ≠ k') :
+      Contains.contains (alter m k f) k' = Contains.contains m k' :=
     LawfulDMapAPI.contains_alter_ne (inst:=DMapAPI_of_MapAPI inst) hne
 
   theorem size_alter_eq_add_one {γ α β} [inst : MapAPI γ α β] [LawfulMapAPI γ α β]
-    {m : γ} {k : α} {f : Option β → Option β}
-    (h : ¬k ∈ m) (h' : (f m[k]?).isSome) :
-    Size.size (alter m k f) = Size.size m + 1 :=
+      {m : γ} {k : α} {f : Option β → Option β}
+      (h : ¬k ∈ m) (h' : (f m[k]?).isSome) :
+      Size.size (alter m k f) = Size.size m + 1 :=
     LawfulDMapAPI.size_alter_eq_add_one (inst:=DMapAPI_of_MapAPI inst) h h'
 
   theorem size_alter_eq_self_of_mem {γ α β} [inst : MapAPI γ α β] [LawfulMapAPI γ α β]
-    {m : γ} {k : α} {f : Option β → Option β}
-    (h : k ∈ m) (h' : (f m[k]?).isSome) :
-    Size.size (alter m k f) = Size.size m :=
+      {m : γ} {k : α} {f : Option β → Option β}
+      (h : k ∈ m) (h' : (f m[k]?).isSome) :
+      Size.size (alter m k f) = Size.size m :=
     LawfulDMapAPI.size_alter_eq_self_of_mem (inst:=DMapAPI_of_MapAPI inst) h h'
 
   theorem size_alter_eq_self_of_not_mem {γ α β} [inst : MapAPI γ α β] [LawfulMapAPI γ α β]
-    {m : γ} {k : α} {f : Option β → Option β}
-    (h : k ∉ m) (h' : (f m[k]?).isNone) :
-    Size.size (alter m k f) = Size.size m :=
+      {m : γ} {k : α} {f : Option β → Option β}
+      (h : k ∉ m) (h' : (f m[k]?).isNone) :
+      Size.size (alter m k f) = Size.size m :=
     LawfulDMapAPI.size_alter_eq_self_of_not_mem (inst:=DMapAPI_of_MapAPI inst) h h'
 
   theorem size_alter_eq_sub_one {γ α β} [inst : MapAPI γ α β] [LawfulMapAPI γ α β]
-    {m : γ} {k : α} {f : Option β → Option β}
-    (h : k ∈ m) (h' : (f m[k]?).isNone) :
-    Size.size (alter m k f) + 1 = Size.size m :=
+      {m : γ} {k : α} {f : Option β → Option β}
+      (h : k ∈ m) (h' : (f m[k]?).isNone) :
+      Size.size (alter m k f) + 1 = Size.size m :=
     LawfulDMapAPI.size_alter_eq_sub_one (inst:=DMapAPI_of_MapAPI inst) h h'
 
   theorem size_alter_le_size {γ α β} [inst : MapAPI γ α β] [LawfulMapAPI γ α β]
-    {m : γ} {k : α} {f : Option β → Option β} :
-    Size.size (alter m k f) ≤ Size.size m + 1 :=
+      {m : γ} {k : α} {f : Option β → Option β} :
+      Size.size (alter m k f) ≤ Size.size m + 1 :=
     LawfulDMapAPI.size_alter_le_size (inst:=DMapAPI_of_MapAPI inst)
 
   theorem size_le_size_alter {γ α β} [inst : MapAPI γ α β] [LawfulMapAPI γ α β]
-    {m : γ} {k : α} {f : Option β → Option β} :
-    Size.size m ≤ Size.size (alter m k f) + 1:=
+      {m : γ} {k : α} {f : Option β → Option β} :
+      Size.size m ≤ Size.size (alter m k f) + 1:=
     LawfulDMapAPI.size_le_size_alter (inst:=DMapAPI_of_MapAPI inst)
 
   theorem isEmpty_alter {γ α β} [inst : MapAPI γ α β] [LawfulMapAPI γ α β]
-    {m : γ} {k : α} {f : Option β → Option β} :
-    IsEmpty.isEmpty (alter m k f) = ((IsEmpty.isEmpty m || Size.size m == 1 && Contains.contains m k) && (f m[k]?).isNone) :=
+      {m : γ} {k : α} {f : Option β → Option β} :
+      IsEmpty.isEmpty (alter m k f) = ((IsEmpty.isEmpty m || Size.size m == 1 && Contains.contains m k) && (f m[k]?).isNone) :=
     LawfulDMapAPI.isEmpty_alter (inst:=DMapAPI_of_MapAPI inst)
 
   theorem isEmpty_alter_eq_isEmpty_erase {γ α β} [inst : MapAPI γ α β] [LawfulMapAPI γ α β]
-    {m : γ} {k : α} {f : Option β → Option β} :
-    IsEmpty.isEmpty (alter m k f) = (IsEmpty.isEmpty (erase (β:=β) m k) && (f m[k]?).isNone) :=
+      {m : γ} {k : α} {f : Option β → Option β} :
+      IsEmpty.isEmpty (alter m k f) = (IsEmpty.isEmpty (erase (β:=β) m k) && (f m[k]?).isNone) :=
     LawfulDMapAPI.isEmpty_alter_eq_isEmpty_erase (inst:=DMapAPI_of_MapAPI inst)
 
   theorem getElem_alter_self {γ α β} [inst : MapAPI γ α β] [LawfulMapAPI γ α β]
-    {m : γ} {k : α} {f : Option β → Option β} {h : k ∈ alter m k f} :
-    (alter m k f)[k]'h = (f m[k]?).get (mem_alter_self.mp h) :=
+      {m : γ} {k : α} {f : Option β → Option β} {h : k ∈ alter m k f} :
+      (alter m k f)[k]'h = (f m[k]?).get (mem_alter_self.mp h) :=
     LawfulDMapAPI.dGetElem_alter_self (inst:=DMapAPI_of_MapAPI inst) (h:=h)
 
   theorem getElem_alter_ne {γ α β} [inst : MapAPI γ α β] [LawfulMapAPI γ α β]
-    {m : γ} {k k' : α} {f : Option β → Option β} {h : k' ∈ alter m k f} (hne : k ≠ k') :
-    (alter m k f)[k']'h = m[k']'((mem_alter_ne hne).mp h) :=
+      {m : γ} {k k' : α} {f : Option β → Option β} {h : k' ∈ alter m k f} (hne : k ≠ k') :
+      (alter m k f)[k']'h = m[k']'((mem_alter_ne hne).mp h) :=
     LawfulDMapAPI.dGetElem_alter_ne (inst:=DMapAPI_of_MapAPI inst) hne
 
   theorem getElem!_alter_self {γ α β} [inst : MapAPI γ α β] [LawfulMapAPI γ α β]
-    {m : γ} {k : α} [Inhabited β] {f : Option β → Option β} :
-    (alter m k f)[k]! = (f m[k]?).get! :=
+      {m : γ} {k : α} [Inhabited β] {f : Option β → Option β} :
+      (alter m k f)[k]! = (f m[k]?).get! :=
     LawfulDMapAPI.dGetElem!_alter_self (inst:=DMapAPI_of_MapAPI inst)
 
   theorem getElem!_alter_ne {γ α β} [inst : MapAPI γ α β] [LawfulMapAPI γ α β]
-    {m : γ} {k k' : α} [Inhabited β] {f : Option β → Option β} (hne : k ≠ k') :
-    (alter m k f)[k']! = m[k']! :=
+      {m : γ} {k k' : α} [Inhabited β] {f : Option β → Option β} (hne : k ≠ k') :
+      (alter m k f)[k']! = m[k']! :=
     LawfulDMapAPI.dGetElem!_alter_ne (inst:=DMapAPI_of_MapAPI inst) hne
 
 end LawfulMapAPI
