ADT/SetLemmas.lean
@@ -12,19 +12,19 @@ open Std
 -/
 
 theorem Std.HashSet.size_zero_iff_forall_not_mem
-  {α} [BEq α] [Hashable α] [EquivBEq α] [LawfulHashable α] {m : HashSet α} : m.size = 0 ↔ ∀ x, x ∉ m := by
+    {α} [BEq α] [Hashable α] [EquivBEq α] [LawfulHashable α] {m : HashSet α} : m.size = 0 ↔ ∀ x, x ∉ m := by
   rw [← HashSet.isEmpty_iff_forall_not_mem, HashSet.isEmpty_eq_size_eq_zero]
   simp
 
 theorem Std.TreeSet.size_zero_iff_forall_not_mem
-  {α} [Ord α] [TransOrd α] {m : TreeSet α} : m.size = 0 ↔ ∀ x, x ∉ m := by
+    {α} [Ord α] [TransOrd α] {m : TreeSet α} : m.size = 0 ↔ ∀ x, x ∉ m := by
   rw [← TreeSet.isEmpty_iff_forall_not_mem, TreeSet.isEmpty_eq_size_eq_zero]
   simp
 
 theorem Std.ExtHashSet.size_zero_iff_forall_not_mem
-  {α} [BEq α] [Hashable α] [EquivBEq α] [LawfulHashable α] {m : ExtHashSet α} : m.size = 0 ↔ ∀ x, x ∉ m := by
+    {α} [BEq α] [Hashable α] [EquivBEq α] [LawfulHashable α] {m : ExtHashSet α} : m.size = 0 ↔ ∀ x, x ∉ m := by
   rw [← ExtHashSet.eq_empty_iff_forall_not_mem, ExtHashSet.eq_empty_iff_size_eq_zero]
 
 theorem Std.ExtTreeSet.size_zero_iff_forall_not_mem
-  {α} [Ord α] [TransOrd α] {m : ExtTreeSet α} : m.size = 0 ↔ ∀ x, x ∉ m := by
+    {α} [Ord α] [TransOrd α] {m : ExtTreeSet α} : m.size = 0 ↔ ∀ x, x ∉ m := by
   rw [← ExtTreeSet.eq_empty_iff_forall_not_mem, ExtTreeSet.eq_empty_iff_size_eq_zero]
